Replaced many contexts with a context record

BananasExpression.thy
@@ -34,8 +34,29 @@ and val =
 | InlV val | InrV val
 | FunV expr
 | InjV name val 
+| VarV name
 
 (* typechecking *)
+
+record static_environment = 
+  var\<^sub>e_type :: "name \<rightharpoonup> type \<times> type" 
+  var\<^sub>v_type :: "name \<rightharpoonup> type" 
+  var\<^sub>t_type :: "name \<rightharpoonup> funct"
+
+definition extend\<^sub>e\<^sub>s :: "name \<Rightarrow> type \<times> type \<Rightarrow> static_environment \<Rightarrow> static_environment" where
+  "extend\<^sub>e\<^sub>s x t \<Gamma> = \<Gamma>\<lparr> var\<^sub>e_type := var\<^sub>e_type \<Gamma>(x \<mapsto> t) \<rparr>"
+
+definition extend\<^sub>v\<^sub>s :: "name \<Rightarrow> type \<Rightarrow> static_environment \<Rightarrow> static_environment" where
+  "extend\<^sub>v\<^sub>s x t \<Gamma> = \<Gamma>\<lparr> var\<^sub>v_type := var\<^sub>v_type \<Gamma>(x \<mapsto> t) \<rparr>"
+
+definition combine\<^sub>s :: "static_environment \<Rightarrow> static_environment \<Rightarrow> static_environment" where
+  "combine\<^sub>s \<Gamma> \<Gamma>' = \<lparr> 
+      var\<^sub>e_type = var\<^sub>e_type \<Gamma> ++ var\<^sub>e_type \<Gamma>', 
+      var\<^sub>v_type = var\<^sub>v_type \<Gamma> ++ var\<^sub>v_type \<Gamma>', 
+      var\<^sub>t_type = var\<^sub>t_type \<Gamma> ++ var\<^sub>t_type \<Gamma>' \<rparr>"
+
+definition domain\<^sub>s :: "static_environment \<Rightarrow> name set" where
+  "domain\<^sub>s \<Gamma> = dom (var\<^sub>e_type \<Gamma>) \<union> dom (var\<^sub>v_type \<Gamma>) \<union> dom (var\<^sub>t_type \<Gamma>)"
 
 fun apply_functor_type :: "type \<Rightarrow> funct \<Rightarrow> type" (infixl "\<star>" 75) where
   "t \<star> Id = t"
@@ -43,72 +64,93 @@ fun apply_functor_type :: "type \<Rightarrow> funct \<Rightarrow> type" (infixl 
 | "t \<star> f\<^sub>1 \<Otimes> f\<^sub>2 = (t \<star> f\<^sub>1) \<otimes> (t \<star> f\<^sub>2)"
 | "t \<star> f\<^sub>1 \<Oplus> f\<^sub>2 = (t \<star> f\<^sub>1) \<oplus> (t \<star> f\<^sub>2)"
 
-inductive typecheck\<^sub>e :: "(name \<rightharpoonup> type \<times> type) \<Rightarrow> (name \<rightharpoonup> funct) \<Rightarrow> expr \<Rightarrow> type \<Rightarrow> type \<Rightarrow> bool" 
-    (infix "& _ \<turnstile> _ : _ \<rightarrow>" 60)
-      and typecheck\<^sub>v :: "(name \<rightharpoonup> type \<times> type) \<Rightarrow> (name \<rightharpoonup> funct) \<Rightarrow> val \<Rightarrow> type \<Rightarrow> bool" 
-    (infix "& _ \<turnstile> _ :" 60) where
-  tc_id [simp]: "\<Gamma> & \<Sigma> \<turnstile> \<epsilon> : t \<rightarrow> t"
-| tc_con [simp]: "\<Gamma> & \<Sigma> \<turnstile> v : t\<^sub>2 \<Longrightarrow> \<Gamma> & \<Sigma> \<turnstile> \<kappa> v : t\<^sub>1 \<rightarrow> t\<^sub>2"
-| tc_comp [simp]: "\<Gamma> & \<Sigma> \<turnstile> f : t\<^sub>2 \<rightarrow> t\<^sub>3 \<Longrightarrow> \<Gamma> & \<Sigma> \<turnstile> g : t\<^sub>1 \<rightarrow> t\<^sub>2 \<Longrightarrow> \<Gamma> & \<Sigma> \<turnstile> f \<cdot> g : t\<^sub>1 \<rightarrow> t\<^sub>3"
-| tc_fst [simp]: "\<Gamma> & \<Sigma> \<turnstile> \<pi>\<^sub>1 : t\<^sub>1 \<otimes> t\<^sub>2 \<rightarrow> t\<^sub>1"
-| tc_snd [simp]: "\<Gamma> & \<Sigma> \<turnstile> \<pi>\<^sub>2 : t\<^sub>1 \<otimes> t\<^sub>2 \<rightarrow> t\<^sub>2"
-| tc_tup [simp]: "\<Gamma> & \<Sigma> \<turnstile> \<Theta> : t \<rightarrow> t \<otimes> t"
-| tc_pair [simp]: "\<Gamma> & \<Sigma> \<turnstile> f\<^sub>1 : t\<^sub>1 \<rightarrow> t\<^sub>2 \<Longrightarrow> \<Gamma> & \<Sigma> \<turnstile> f\<^sub>2 : t\<^sub>3 \<rightarrow> t\<^sub>4 \<Longrightarrow> 
-    \<Gamma> & \<Sigma> \<turnstile> f\<^sub>1 \<parallel> f\<^sub>2 : t\<^sub>1 \<otimes> t\<^sub>3 \<rightarrow> t\<^sub>2 \<otimes> t\<^sub>4"
-| tc_inl [simp]: "\<Gamma> & \<Sigma> \<turnstile> \<iota>\<^sub>l : t\<^sub>1 \<rightarrow> t\<^sub>1 \<oplus> t\<^sub>2"
-| tc_inr [simp]: "\<Gamma> & \<Sigma> \<turnstile> \<iota>\<^sub>r : t\<^sub>2 \<rightarrow> t\<^sub>1 \<oplus> t\<^sub>2"
-| tc_str [simp]: "\<Gamma> & \<Sigma> \<turnstile> \<Xi> : t\<^sub>1 \<oplus> t\<^sub>1 \<rightarrow> t\<^sub>1"
-| tc_case [simp]: "\<Gamma> & \<Sigma> \<turnstile> f\<^sub>l : t\<^sub>1 \<rightarrow> t\<^sub>3 \<Longrightarrow> \<Gamma> & \<Sigma> \<turnstile> f\<^sub>r : t\<^sub>2 \<rightarrow> t\<^sub>4 \<Longrightarrow> 
-    \<Gamma> & \<Sigma> \<turnstile> f\<^sub>l \<bar> f\<^sub>r : t\<^sub>1 \<oplus> t\<^sub>2 \<rightarrow> t\<^sub>3 \<oplus> t\<^sub>4"
-| tc_dst [simp]: "\<Gamma> & \<Sigma> \<turnstile> \<rhd> : (t\<^sub>1 \<oplus> t\<^sub>2) \<otimes> t\<^sub>3 \<rightarrow> t\<^sub>1 \<otimes> t\<^sub>3 \<oplus> t\<^sub>2 \<otimes> t\<^sub>3"
-| tc_app [simp]: "\<Gamma> & \<Sigma> \<turnstile> $ : (t\<^sub>1 \<hookrightarrow> t\<^sub>2) \<otimes> t\<^sub>1 \<rightarrow> t\<^sub>2"
-| tc_arr [simp]: "\<Gamma> & \<Sigma> \<turnstile> f : t\<^sub>1 \<rightarrow> t\<^sub>2 \<Longrightarrow> \<Gamma> & \<Sigma> \<turnstile> g : t\<^sub>3 \<rightarrow> t\<^sub>4 \<Longrightarrow> 
-    \<Gamma> & \<Sigma> \<turnstile> g \<leftarrow> f : t\<^sub>2 \<hookrightarrow> t\<^sub>3 \<rightarrow> t\<^sub>1 \<hookrightarrow> t\<^sub>4"
-| tc_inj [simp]: "\<Sigma> n = Some F \<Longrightarrow> \<Gamma> & \<Sigma> \<turnstile> \<succ>\<^bsub>n\<^esub> : \<mu> F \<star> F \<rightarrow> \<mu> F"
-| tc_outj [simp]: "\<Sigma> n = Some F \<Longrightarrow> \<Gamma> & \<Sigma> \<turnstile> \<prec>\<^bsub>n\<^esub> : \<mu> F \<rightarrow> \<mu> F \<star> F"
-| tc_cata [simp]: "\<Sigma> n = Some F \<Longrightarrow> \<Gamma> & \<Sigma> \<turnstile> f : t \<star> F \<rightarrow> t \<Longrightarrow> \<Gamma> & \<Sigma> \<turnstile> \<lparr> f \<rparr>\<^bsub>n\<^esub> : \<mu> F \<rightarrow> t"
-| tc_ana [simp]: "\<Sigma> n = Some F \<Longrightarrow> \<Gamma> & \<Sigma> \<turnstile> f : t \<rightarrow> t \<star> F \<Longrightarrow> \<Gamma> & \<Sigma> \<turnstile> \<lbrakk> f \<rbrakk>\<^bsub>n\<^esub> : t \<rightarrow> \<mu> F"
-| tc_var [simp]: "\<Gamma> x = Some (t\<^sub>1, t\<^sub>2) \<Longrightarrow> \<Gamma> & \<Sigma> \<turnstile> Var x : t\<^sub>1 \<rightarrow> t\<^sub>2"
+inductive typecheck\<^sub>e :: "static_environment \<Rightarrow> expr \<Rightarrow> type \<Rightarrow> type \<Rightarrow> bool" (infix "\<turnstile> _ : _ \<rightarrow>" 60)
+      and typecheck\<^sub>v :: "static_environment \<Rightarrow> val \<Rightarrow> type \<Rightarrow> bool" (infix "\<turnstile> _ :" 60) where
+  tc_id [simp]: "\<Gamma> \<turnstile> \<epsilon> : t \<rightarrow> t"
+| tc_con [simp]: "\<Gamma> \<turnstile> v : t\<^sub>2 \<Longrightarrow> \<Gamma> \<turnstile> \<kappa> v : t\<^sub>1 \<rightarrow> t\<^sub>2"
+| tc_comp [simp]: "\<Gamma> \<turnstile> f : t\<^sub>2 \<rightarrow> t\<^sub>3 \<Longrightarrow> \<Gamma> \<turnstile> g : t\<^sub>1 \<rightarrow> t\<^sub>2 \<Longrightarrow> \<Gamma> \<turnstile> f \<cdot> g : t\<^sub>1 \<rightarrow> t\<^sub>3"
+| tc_fst [simp]: "\<Gamma> \<turnstile> \<pi>\<^sub>1 : t\<^sub>1 \<otimes> t\<^sub>2 \<rightarrow> t\<^sub>1"
+| tc_snd [simp]: "\<Gamma> \<turnstile> \<pi>\<^sub>2 : t\<^sub>1 \<otimes> t\<^sub>2 \<rightarrow> t\<^sub>2"
+| tc_tup [simp]: "\<Gamma> \<turnstile> \<Theta> : t \<rightarrow> t \<otimes> t"
+| tc_pair [simp]: "\<Gamma> \<turnstile> f\<^sub>1 : t\<^sub>1 \<rightarrow> t\<^sub>2 \<Longrightarrow> \<Gamma> \<turnstile> f\<^sub>2 : t\<^sub>3 \<rightarrow> t\<^sub>4 \<Longrightarrow> 
+    \<Gamma> \<turnstile> f\<^sub>1 \<parallel> f\<^sub>2 : t\<^sub>1 \<otimes> t\<^sub>3 \<rightarrow> t\<^sub>2 \<otimes> t\<^sub>4"
+| tc_inl [simp]: "\<Gamma> \<turnstile> \<iota>\<^sub>l : t\<^sub>1 \<rightarrow> t\<^sub>1 \<oplus> t\<^sub>2"
+| tc_inr [simp]: "\<Gamma> \<turnstile> \<iota>\<^sub>r : t\<^sub>2 \<rightarrow> t\<^sub>1 \<oplus> t\<^sub>2"
+| tc_str [simp]: "\<Gamma> \<turnstile> \<Xi> : t\<^sub>1 \<oplus> t\<^sub>1 \<rightarrow> t\<^sub>1"
+| tc_case [simp]: "\<Gamma> \<turnstile> f\<^sub>l : t\<^sub>1 \<rightarrow> t\<^sub>3 \<Longrightarrow> \<Gamma> \<turnstile> f\<^sub>r : t\<^sub>2 \<rightarrow> t\<^sub>4 \<Longrightarrow> 
+    \<Gamma> \<turnstile> f\<^sub>l \<bar> f\<^sub>r : t\<^sub>1 \<oplus> t\<^sub>2 \<rightarrow> t\<^sub>3 \<oplus> t\<^sub>4"
+| tc_dst [simp]: "\<Gamma> \<turnstile> \<rhd> : (t\<^sub>1 \<oplus> t\<^sub>2) \<otimes> t\<^sub>3 \<rightarrow> t\<^sub>1 \<otimes> t\<^sub>3 \<oplus> t\<^sub>2 \<otimes> t\<^sub>3"
+| tc_app [simp]: "\<Gamma> \<turnstile> $ : (t\<^sub>1 \<hookrightarrow> t\<^sub>2) \<otimes> t\<^sub>1 \<rightarrow> t\<^sub>2"
+| tc_arr [simp]: "\<Gamma> \<turnstile> f : t\<^sub>1 \<rightarrow> t\<^sub>2 \<Longrightarrow> \<Gamma> \<turnstile> g : t\<^sub>3 \<rightarrow> t\<^sub>4 \<Longrightarrow> 
+    \<Gamma> \<turnstile> g \<leftarrow> f : t\<^sub>2 \<hookrightarrow> t\<^sub>3 \<rightarrow> t\<^sub>1 \<hookrightarrow> t\<^sub>4"
+| tc_inj [simp]: "var\<^sub>t_type \<Gamma> n = Some F \<Longrightarrow> \<Gamma> \<turnstile> \<succ>\<^bsub>n\<^esub> : \<mu> F \<star> F \<rightarrow> \<mu> F"
+| tc_outj [simp]: "var\<^sub>t_type \<Gamma> n = Some F \<Longrightarrow> \<Gamma> \<turnstile> \<prec>\<^bsub>n\<^esub> : \<mu> F \<rightarrow> \<mu> F \<star> F"
+| tc_cata [simp]: "var\<^sub>t_type \<Gamma> n = Some F \<Longrightarrow> \<Gamma> \<turnstile> f : t \<star> F \<rightarrow> t \<Longrightarrow> \<Gamma> \<turnstile> \<lparr> f \<rparr>\<^bsub>n\<^esub> : \<mu> F \<rightarrow> t"
+| tc_ana [simp]: "var\<^sub>t_type \<Gamma> n = Some F \<Longrightarrow> \<Gamma> \<turnstile> f : t \<rightarrow> t \<star> F \<Longrightarrow> \<Gamma> \<turnstile> \<lbrakk> f \<rbrakk>\<^bsub>n\<^esub> : t \<rightarrow> \<mu> F"
+| tc_var [simp]: "var\<^sub>e_type \<Gamma> x = Some (t\<^sub>1, t\<^sub>2) \<Longrightarrow> \<Gamma> \<turnstile> Var x : t\<^sub>1 \<rightarrow> t\<^sub>2"
 
-| tcv_unit [simp]: "\<Gamma> & \<Sigma> \<turnstile> UnitV : \<one>"
-| tcv_pair [simp]: "\<Gamma> & \<Sigma> \<turnstile> v\<^sub>1 : t\<^sub>1 \<Longrightarrow> \<Gamma> & \<Sigma> \<turnstile> v\<^sub>2 : t\<^sub>2 \<Longrightarrow> \<Gamma> & \<Sigma> \<turnstile> PairV v\<^sub>1 v\<^sub>2 : t\<^sub>1 \<otimes> t\<^sub>2"
-| tcv_inl [simp]: "\<Gamma> & \<Sigma> \<turnstile> v : t\<^sub>1 \<Longrightarrow> \<Gamma> & \<Sigma> \<turnstile> InlV v : t\<^sub>1 \<oplus> t\<^sub>2"
-| tcv_inr [simp]: "\<Gamma> & \<Sigma> \<turnstile> v : t\<^sub>2 \<Longrightarrow> \<Gamma> & \<Sigma> \<turnstile> InrV v : t\<^sub>1 \<oplus> t\<^sub>2"
-| tcv_fun [simp]: "\<Gamma> & \<Sigma> \<turnstile> e : t\<^sub>1 \<rightarrow> t\<^sub>2 \<Longrightarrow> \<Gamma> & \<Sigma> \<turnstile> FunV e : t\<^sub>1 \<hookrightarrow> t\<^sub>2"
-| tcv_inj [simp]: "\<Sigma> n = Some F \<Longrightarrow> \<Gamma> & \<Sigma> \<turnstile> v : \<mu> F \<star> F \<Longrightarrow> \<Gamma> & \<Sigma> \<turnstile> InjV n v : \<mu> F"
+| tcv_unit [simp]: "\<Gamma> \<turnstile> UnitV : \<one>"
+| tcv_pair [simp]: "\<Gamma> \<turnstile> v\<^sub>1 : t\<^sub>1 \<Longrightarrow> \<Gamma> \<turnstile> v\<^sub>2 : t\<^sub>2 \<Longrightarrow> \<Gamma> \<turnstile> PairV v\<^sub>1 v\<^sub>2 : t\<^sub>1 \<otimes> t\<^sub>2"
+| tcv_inl [simp]: "\<Gamma> \<turnstile> v : t\<^sub>1 \<Longrightarrow> \<Gamma> \<turnstile> InlV v : t\<^sub>1 \<oplus> t\<^sub>2"
+| tcv_inr [simp]: "\<Gamma> \<turnstile> v : t\<^sub>2 \<Longrightarrow> \<Gamma> \<turnstile> InrV v : t\<^sub>1 \<oplus> t\<^sub>2"
+| tcv_fun [simp]: "\<Gamma> \<turnstile> e : t\<^sub>1 \<rightarrow> t\<^sub>2 \<Longrightarrow> \<Gamma> \<turnstile> FunV e : t\<^sub>1 \<hookrightarrow> t\<^sub>2"
+| tcv_inj [simp]: "var\<^sub>t_type \<Gamma> n = Some F \<Longrightarrow> \<Gamma> \<turnstile> v : \<mu> F \<star> F \<Longrightarrow> \<Gamma> \<turnstile> InjV n v : \<mu> F"
 
-inductive_cases [elim]: "\<Gamma> & \<Sigma> \<turnstile> \<epsilon> : t \<rightarrow> t'"
-inductive_cases [elim]: "\<Gamma> & \<Sigma> \<turnstile> \<kappa> v : t \<rightarrow> t'"
-inductive_cases [elim]: "\<Gamma> & \<Sigma> \<turnstile> f \<cdot> g : t \<rightarrow> t'"
-inductive_cases [elim]: "\<Gamma> & \<Sigma> \<turnstile> \<pi>\<^sub>1 : t \<rightarrow> t'"
-inductive_cases [elim]: "\<Gamma> & \<Sigma> \<turnstile> \<pi>\<^sub>2 : t \<rightarrow> t'"
-inductive_cases [elim]: "\<Gamma> & \<Sigma> \<turnstile> \<Theta> : t \<rightarrow> t'"
-inductive_cases [elim]: "\<Gamma> & \<Sigma> \<turnstile> f\<^sub>l \<parallel> f\<^sub>r : t \<rightarrow> t'"
-inductive_cases [elim]: "\<Gamma> & \<Sigma> \<turnstile> \<iota>\<^sub>l : t \<rightarrow> t'"
-inductive_cases [elim]: "\<Gamma> & \<Sigma> \<turnstile> \<iota>\<^sub>r : t \<rightarrow> t'"
-inductive_cases [elim]: "\<Gamma> & \<Sigma> \<turnstile> \<Xi> : t \<rightarrow> t'"
-inductive_cases [elim]: "\<Gamma> & \<Sigma> \<turnstile> f\<^sub>l \<bar> f\<^sub>r : t \<rightarrow> t'"
-inductive_cases [elim]: "\<Gamma> & \<Sigma> \<turnstile> \<rhd> : t \<rightarrow> t'"
-inductive_cases [elim]: "\<Gamma> & \<Sigma> \<turnstile> $ : t \<rightarrow> t'"
-inductive_cases [elim]: "\<Gamma> & \<Sigma> \<turnstile> g \<leftarrow> f : t \<rightarrow> t'"
-inductive_cases [elim]: "\<Gamma> & \<Sigma> \<turnstile> \<prec>\<^bsub>F\<^esub> : t \<rightarrow> t'"
-inductive_cases [elim]: "\<Gamma> & \<Sigma> \<turnstile> \<succ>\<^bsub>F\<^esub> : t \<rightarrow> t'"
-inductive_cases [elim]: "\<Gamma> & \<Sigma> \<turnstile> \<lparr> f \<rparr>\<^bsub>F\<^esub> : t \<rightarrow> t'"
-inductive_cases [elim]: "\<Gamma> & \<Sigma> \<turnstile> \<lbrakk> f \<rbrakk>\<^bsub>F\<^esub> : t \<rightarrow> t'"
-inductive_cases [elim]: "\<Gamma> & \<Sigma> \<turnstile> Var x : t \<rightarrow> t'"
+inductive_cases [elim]: "\<Gamma> \<turnstile> \<epsilon> : t \<rightarrow> t'"
+inductive_cases [elim]: "\<Gamma> \<turnstile> \<kappa> v : t \<rightarrow> t'"
+inductive_cases [elim]: "\<Gamma> \<turnstile> f \<cdot> g : t \<rightarrow> t'"
+inductive_cases [elim]: "\<Gamma> \<turnstile> \<pi>\<^sub>1 : t \<rightarrow> t'"
+inductive_cases [elim]: "\<Gamma> \<turnstile> \<pi>\<^sub>2 : t \<rightarrow> t'"
+inductive_cases [elim]: "\<Gamma> \<turnstile> \<Theta> : t \<rightarrow> t'"
+inductive_cases [elim]: "\<Gamma> \<turnstile> f\<^sub>l \<parallel> f\<^sub>r : t \<rightarrow> t'"
+inductive_cases [elim]: "\<Gamma> \<turnstile> \<iota>\<^sub>l : t \<rightarrow> t'"
+inductive_cases [elim]: "\<Gamma> \<turnstile> \<iota>\<^sub>r : t \<rightarrow> t'"
+inductive_cases [elim]: "\<Gamma> \<turnstile> \<Xi> : t \<rightarrow> t'"
+inductive_cases [elim]: "\<Gamma> \<turnstile> f\<^sub>l \<bar> f\<^sub>r : t \<rightarrow> t'"
+inductive_cases [elim]: "\<Gamma> \<turnstile> \<rhd> : t \<rightarrow> t'"
+inductive_cases [elim]: "\<Gamma> \<turnstile> $ : t \<rightarrow> t'"
+inductive_cases [elim]: "\<Gamma> \<turnstile> g \<leftarrow> f : t \<rightarrow> t'"
+inductive_cases [elim]: "\<Gamma> \<turnstile> \<prec>\<^bsub>n\<^esub> : t \<rightarrow> t'"
+inductive_cases [elim]: "\<Gamma> \<turnstile> \<succ>\<^bsub>n\<^esub> : t \<rightarrow> t'"
+inductive_cases [elim]: "\<Gamma> \<turnstile> \<lparr> f \<rparr>\<^bsub>n\<^esub> : t \<rightarrow> t'"
+inductive_cases [elim]: "\<Gamma> \<turnstile> \<lbrakk> f \<rbrakk>\<^bsub>n\<^esub> : t \<rightarrow> t'"
+inductive_cases [elim]: "\<Gamma> \<turnstile> Var x : t \<rightarrow> t'"
 
-inductive_cases [elim]: "\<Gamma> & \<Sigma> \<turnstile> UnitV : t"
-inductive_cases [elim]: "\<Gamma> & \<Sigma> \<turnstile> PairV v\<^sub>1 v\<^sub>2 : t"
-inductive_cases [elim]: "\<Gamma> & \<Sigma> \<turnstile> InrV v : t"
-inductive_cases [elim]: "\<Gamma> & \<Sigma> \<turnstile> InlV v : t"
-inductive_cases [elim]: "\<Gamma> & \<Sigma> \<turnstile> FunV e : t"
-inductive_cases [elim]: "\<Gamma> & \<Sigma> \<turnstile> InjV f v : t"
-
-definition typecheck_context :: "(name \<rightharpoonup> type \<times> type) \<Rightarrow> (name \<rightharpoonup> funct) \<Rightarrow> (name \<rightharpoonup> expr) \<Rightarrow> bool" 
-    (infix "& _ \<tturnstile>" 60) where
-  "(\<Gamma> & \<Sigma> \<tturnstile> \<Lambda>) = (\<forall>x t\<^sub>1 t\<^sub>2. \<Gamma> x = Some (t\<^sub>1, t\<^sub>2) \<longrightarrow> (\<exists>e. \<Lambda> x = Some e \<and> \<Gamma> & \<Sigma> \<turnstile> e : t\<^sub>1 \<rightarrow> t\<^sub>2))"
+inductive_cases [elim]: "\<Gamma> \<turnstile> UnitV : t"
+inductive_cases [elim]: "\<Gamma> \<turnstile> PairV v\<^sub>1 v\<^sub>2 : t"
+inductive_cases [elim]: "\<Gamma> \<turnstile> InrV v : t"
+inductive_cases [elim]: "\<Gamma> \<turnstile> InlV v : t"
+inductive_cases [elim]: "\<Gamma> \<turnstile> FunV e : t"
+inductive_cases [elim]: "\<Gamma> \<turnstile> InjV f v : t"
 
 (* evaluation *)
+
+record dynamic_environment = 
+  var\<^sub>e_bind :: "name \<rightharpoonup> expr" 
+  var\<^sub>v_bind :: "name \<rightharpoonup> val" 
+  var\<^sub>t_bind :: "name \<rightharpoonup> funct"
+
+definition extend\<^sub>e\<^sub>d :: "name \<Rightarrow> expr \<Rightarrow> dynamic_environment \<Rightarrow> dynamic_environment" where
+  "extend\<^sub>e\<^sub>d x t \<Lambda> = \<Lambda>\<lparr> var\<^sub>e_bind := var\<^sub>e_bind \<Lambda>(x \<mapsto> t) \<rparr>"
+
+definition extend\<^sub>v\<^sub>d :: "name \<Rightarrow> val \<Rightarrow> dynamic_environment \<Rightarrow> dynamic_environment" where
+  "extend\<^sub>v\<^sub>d x t \<Lambda> = \<Lambda>\<lparr> var\<^sub>v_bind := var\<^sub>v_bind \<Lambda>(x \<mapsto> t) \<rparr>"
+
+definition combine\<^sub>d :: "dynamic_environment \<Rightarrow> dynamic_environment \<Rightarrow> dynamic_environment" where
+  "combine\<^sub>d \<Lambda> \<Lambda>' = \<lparr> 
+      var\<^sub>e_bind = var\<^sub>e_bind \<Lambda> ++ var\<^sub>e_bind \<Lambda>', 
+      var\<^sub>v_bind = var\<^sub>v_bind \<Lambda> ++ var\<^sub>v_bind \<Lambda>', 
+      var\<^sub>t_bind = var\<^sub>t_bind \<Lambda> ++ var\<^sub>t_bind \<Lambda>' \<rparr>"
+
+definition domain\<^sub>d :: "dynamic_environment \<Rightarrow> name set" where
+  "domain\<^sub>d \<Lambda> = dom (var\<^sub>e_bind \<Lambda>) \<union> dom (var\<^sub>v_bind \<Lambda>) \<union> dom (var\<^sub>t_bind \<Lambda>)"
+
+definition typecheck_environment :: "static_environment \<Rightarrow> dynamic_environment \<Rightarrow> bool" 
+    (infix "\<tturnstile>" 60) where
+  "\<Gamma> \<tturnstile> \<Lambda> = (var\<^sub>t_type \<Gamma> = var\<^sub>t_bind \<Lambda> \<and> dom (var\<^sub>e_type \<Gamma>) = dom (var\<^sub>e_bind \<Lambda>) \<and> 
+    dom (var\<^sub>t_type \<Gamma>) = dom (var\<^sub>t_bind \<Lambda>) \<and> 
+      (\<forall>x t\<^sub>1 t\<^sub>2. var\<^sub>e_type \<Gamma> x = Some (t\<^sub>1, t\<^sub>2) \<longrightarrow> (\<exists>e. var\<^sub>e_bind \<Lambda> x = Some e \<and> \<Gamma> \<turnstile> e : t\<^sub>1 \<rightarrow> t\<^sub>2)) \<and>
+        (\<forall>x t. var\<^sub>v_type \<Gamma> x = Some t \<longrightarrow> (\<exists>v. var\<^sub>v_bind \<Lambda> x = Some v \<and> \<Gamma> \<turnstile> v : t)))"
 
 fun apply_functor_expr :: "expr \<Rightarrow> funct \<Rightarrow> expr" (infixl "\<bullet>" 75) where
   "e \<bullet> Id = e"
@@ -116,86 +158,85 @@ fun apply_functor_expr :: "expr \<Rightarrow> funct \<Rightarrow> expr" (infixl 
 | "e \<bullet> f\<^sub>1 \<Otimes> f\<^sub>2 = (e \<bullet> f\<^sub>1) \<parallel> (e \<bullet> f\<^sub>2)"
 | "e \<bullet> f\<^sub>1 \<Oplus> f\<^sub>2 = (e \<bullet> f\<^sub>1) \<bar> (e \<bullet> f\<^sub>2)"
 
-inductive evaluate :: "(name \<rightharpoonup> expr) \<Rightarrow> (name \<rightharpoonup> funct) \<Rightarrow> expr \<Rightarrow> val \<Rightarrow> expr \<Rightarrow> val \<Rightarrow> bool" 
-    (infix "& _ \<turnstile> _ \<cdot> _ \<leadsto> _ \<cdot>" 60) where
-  ev_con [simp]: "\<Lambda> & \<Sigma> \<turnstile> \<kappa> v\<^sub>1 \<cdot> v\<^sub>2 \<leadsto> \<epsilon> \<cdot> v\<^sub>1"
-| ev_comp1 [simp]: "\<Lambda> & \<Sigma> \<turnstile> g \<cdot> v \<leadsto> g' \<cdot> v' \<Longrightarrow> \<Lambda> & \<Sigma> \<turnstile> (f \<cdot> g) \<cdot> v \<leadsto> (f \<cdot> g') \<cdot> v'"
-| ev_comp2 [simp]: "\<Lambda> & \<Sigma> \<turnstile> (f \<cdot> \<epsilon>) \<cdot> v \<leadsto> f \<cdot> v"
-| ev_fst [simp]: "\<Lambda> & \<Sigma> \<turnstile> \<pi>\<^sub>1 \<cdot> PairV v\<^sub>1 v\<^sub>2 \<leadsto> \<epsilon> \<cdot> v\<^sub>1"
-| ev_snd [simp]: "\<Lambda> & \<Sigma> \<turnstile> \<pi>\<^sub>2 \<cdot> PairV v\<^sub>1 v\<^sub>2 \<leadsto> \<epsilon> \<cdot> v\<^sub>2"
-| ev_pair1 [simp]: "\<Lambda> & \<Sigma> \<turnstile> f\<^sub>1 \<cdot> v\<^sub>1 \<leadsto> f\<^sub>1' \<cdot> v\<^sub>1' \<Longrightarrow> 
-    \<Lambda> & \<Sigma> \<turnstile> f\<^sub>1 \<parallel> f\<^sub>2 \<cdot> PairV v\<^sub>1 v\<^sub>2 \<leadsto> f\<^sub>1' \<parallel> f\<^sub>2 \<cdot> PairV v\<^sub>1' v\<^sub>2"
-| ev_pair2 [simp]: "\<Lambda> & \<Sigma> \<turnstile> f\<^sub>2 \<cdot> v\<^sub>2 \<leadsto> f\<^sub>2' \<cdot> v\<^sub>2' \<Longrightarrow> 
-    \<Lambda> & \<Sigma> \<turnstile> \<epsilon> \<parallel> f\<^sub>2 \<cdot> PairV v\<^sub>1 v\<^sub>2 \<leadsto> \<epsilon> \<parallel> f\<^sub>2' \<cdot> PairV v\<^sub>1 v\<^sub>2'"
-| ev_pair3 [simp]: "\<Lambda> & \<Sigma> \<turnstile> \<epsilon> \<parallel> \<epsilon> \<cdot> PairV v\<^sub>1 v\<^sub>2 \<leadsto> \<epsilon> \<cdot> PairV v\<^sub>1 v\<^sub>2"
-| ev_tup [simp]: "\<Lambda> & \<Sigma> \<turnstile> \<Theta> \<cdot> v \<leadsto> \<epsilon> \<cdot> PairV v v"
-| ev_inl [simp]: "\<Lambda> & \<Sigma> \<turnstile> \<iota>\<^sub>l \<cdot> v \<leadsto> \<epsilon> \<cdot> InlV v"
-| ev_inr [simp]: "\<Lambda> & \<Sigma> \<turnstile> \<iota>\<^sub>r \<cdot> v \<leadsto> \<epsilon> \<cdot> InrV v"
-| ev_strl [simp]: "\<Lambda> & \<Sigma> \<turnstile> \<Xi> \<cdot> InlV v \<leadsto> \<epsilon> \<cdot> v"
-| ev_strr [simp]: "\<Lambda> & \<Sigma> \<turnstile> \<Xi> \<cdot> InrV v \<leadsto> \<epsilon> \<cdot> v"
-| ev_csl [simp]: "\<Lambda> & \<Sigma> \<turnstile> f\<^sub>l \<bar> f\<^sub>r \<cdot> InlV v \<leadsto> (\<iota>\<^sub>l \<cdot> f\<^sub>l) \<cdot> v"
-| ev_csr [simp]: "\<Lambda> & \<Sigma> \<turnstile> f\<^sub>l \<bar> f\<^sub>r \<cdot> InrV v \<leadsto> (\<iota>\<^sub>r \<cdot> f\<^sub>r) \<cdot> v"
-| ev_dstl [simp]: "\<Lambda> & \<Sigma> \<turnstile> \<rhd> \<cdot> PairV (InlV v\<^sub>1) v\<^sub>2 \<leadsto> \<epsilon> \<cdot> InlV (PairV v\<^sub>1 v\<^sub>2)"
-| ev_dstr [simp]: "\<Lambda> & \<Sigma> \<turnstile> \<rhd> \<cdot> PairV (InrV v\<^sub>1) v\<^sub>2 \<leadsto> \<epsilon> \<cdot> InrV (PairV v\<^sub>1 v\<^sub>2)"
-| ev_app [simp]: "\<Lambda> & \<Sigma> \<turnstile> $ \<cdot> PairV (FunV e) v \<leadsto> e \<cdot> v"
-| ev_arr [simp]: "\<Lambda> & \<Sigma> \<turnstile> g \<leftarrow> f \<cdot> FunV e \<leadsto> \<epsilon> \<cdot> FunV (g \<cdot> e \<cdot> f)"
-| ev_inj [simp]: "\<Lambda> & \<Sigma> \<turnstile> \<succ>\<^bsub>n\<^esub> \<cdot> v \<leadsto> \<epsilon> \<cdot> InjV n v"
+inductive evaluate :: "dynamic_environment \<Rightarrow> expr \<Rightarrow> val \<Rightarrow> expr \<Rightarrow> val \<Rightarrow> bool" 
+    (infix "\<turnstile> _ \<cdot> _ \<leadsto> _ \<cdot>" 60) where
+  ev_con [simp]: "\<Lambda> \<turnstile> \<kappa> v\<^sub>1 \<cdot> v\<^sub>2 \<leadsto> \<epsilon> \<cdot> v\<^sub>1"
+| ev_comp1 [simp]: "\<Lambda> \<turnstile> g \<cdot> v \<leadsto> g' \<cdot> v' \<Longrightarrow> \<Lambda> \<turnstile> (f \<cdot> g) \<cdot> v \<leadsto> (f \<cdot> g') \<cdot> v'"
+| ev_comp2 [simp]: "\<Lambda> \<turnstile> (f \<cdot> \<epsilon>) \<cdot> v \<leadsto> f \<cdot> v"
+| ev_fst [simp]: "\<Lambda> \<turnstile> \<pi>\<^sub>1 \<cdot> PairV v\<^sub>1 v\<^sub>2 \<leadsto> \<epsilon> \<cdot> v\<^sub>1"
+| ev_snd [simp]: "\<Lambda> \<turnstile> \<pi>\<^sub>2 \<cdot> PairV v\<^sub>1 v\<^sub>2 \<leadsto> \<epsilon> \<cdot> v\<^sub>2"
+| ev_pair1 [simp]: "\<Lambda> \<turnstile> f\<^sub>1 \<cdot> v\<^sub>1 \<leadsto> f\<^sub>1' \<cdot> v\<^sub>1' \<Longrightarrow> 
+    \<Lambda> \<turnstile> f\<^sub>1 \<parallel> f\<^sub>2 \<cdot> PairV v\<^sub>1 v\<^sub>2 \<leadsto> f\<^sub>1' \<parallel> f\<^sub>2 \<cdot> PairV v\<^sub>1' v\<^sub>2"
+| ev_pair2 [simp]: "\<Lambda> \<turnstile> f\<^sub>2 \<cdot> v\<^sub>2 \<leadsto> f\<^sub>2' \<cdot> v\<^sub>2' \<Longrightarrow> 
+    \<Lambda> \<turnstile> \<epsilon> \<parallel> f\<^sub>2 \<cdot> PairV v\<^sub>1 v\<^sub>2 \<leadsto> \<epsilon> \<parallel> f\<^sub>2' \<cdot> PairV v\<^sub>1 v\<^sub>2'"
+| ev_pair3 [simp]: "\<Lambda> \<turnstile> \<epsilon> \<parallel> \<epsilon> \<cdot> PairV v\<^sub>1 v\<^sub>2 \<leadsto> \<epsilon> \<cdot> PairV v\<^sub>1 v\<^sub>2"
+| ev_tup [simp]: "\<Lambda> \<turnstile> \<Theta> \<cdot> v \<leadsto> \<epsilon> \<cdot> PairV v v"
+| ev_inl [simp]: "\<Lambda> \<turnstile> \<iota>\<^sub>l \<cdot> v \<leadsto> \<epsilon> \<cdot> InlV v"
+| ev_inr [simp]: "\<Lambda> \<turnstile> \<iota>\<^sub>r \<cdot> v \<leadsto> \<epsilon> \<cdot> InrV v"
+| ev_strl [simp]: "\<Lambda> \<turnstile> \<Xi> \<cdot> InlV v \<leadsto> \<epsilon> \<cdot> v"
+| ev_strr [simp]: "\<Lambda> \<turnstile> \<Xi> \<cdot> InrV v \<leadsto> \<epsilon> \<cdot> v"
+| ev_csl [simp]: "\<Lambda> \<turnstile> f\<^sub>l \<bar> f\<^sub>r \<cdot> InlV v \<leadsto> (\<iota>\<^sub>l \<cdot> f\<^sub>l) \<cdot> v"
+| ev_csr [simp]: "\<Lambda> \<turnstile> f\<^sub>l \<bar> f\<^sub>r \<cdot> InrV v \<leadsto> (\<iota>\<^sub>r \<cdot> f\<^sub>r) \<cdot> v"
+| ev_dstl [simp]: "\<Lambda> \<turnstile> \<rhd> \<cdot> PairV (InlV v\<^sub>1) v\<^sub>2 \<leadsto> \<epsilon> \<cdot> InlV (PairV v\<^sub>1 v\<^sub>2)"
+| ev_dstr [simp]: "\<Lambda> \<turnstile> \<rhd> \<cdot> PairV (InrV v\<^sub>1) v\<^sub>2 \<leadsto> \<epsilon> \<cdot> InrV (PairV v\<^sub>1 v\<^sub>2)"
+| ev_app [simp]: "\<Lambda> \<turnstile> $ \<cdot> PairV (FunV e) v \<leadsto> e \<cdot> v"
+| ev_arr [simp]: "\<Lambda> \<turnstile> g \<leftarrow> f \<cdot> FunV e \<leadsto> \<epsilon> \<cdot> FunV (g \<cdot> e \<cdot> f)"
+| ev_inj [simp]: "\<Lambda> \<turnstile> \<succ>\<^bsub>n\<^esub> \<cdot> v \<leadsto> \<epsilon> \<cdot> InjV n v"
 (* Should have n = m, but makes progress harder. Also, typechecking guarantees it.  *)
-| ev_outj [simp]: "\<Lambda> & \<Sigma> \<turnstile> \<prec>\<^bsub>n\<^esub> \<cdot> InjV m v \<leadsto> \<epsilon> \<cdot> v" 
-| ev_cata [simp]: "\<Sigma> n = Some F \<Longrightarrow> \<Lambda> & \<Sigma> \<turnstile> \<lparr> f \<rparr>\<^bsub>n\<^esub> \<cdot> v \<leadsto> (f \<cdot> \<lparr> f \<rparr>\<^bsub>n\<^esub> \<bullet> F \<cdot> \<prec>\<^bsub>n\<^esub>) \<cdot> v"
-| ev_ana [simp]: "\<Sigma> n = Some F \<Longrightarrow> \<Lambda> & \<Sigma> \<turnstile> \<lbrakk> f \<rbrakk>\<^bsub>n\<^esub> \<cdot> v \<leadsto> (\<succ>\<^bsub>n\<^esub> \<cdot> \<lbrakk> f \<rbrakk>\<^bsub>n\<^esub> \<bullet> F \<cdot> f) \<cdot> v"
-| ev_var [simp]: "\<Lambda> x = Some e \<Longrightarrow> \<Lambda> & \<Sigma> \<turnstile> Var x \<cdot> v \<leadsto> e \<cdot> v"
+| ev_outj [simp]: "\<Lambda> \<turnstile> \<prec>\<^bsub>n\<^esub> \<cdot> InjV m v \<leadsto> \<epsilon> \<cdot> v" 
+| ev_cata [simp]: "var\<^sub>t_bind \<Lambda> n = Some F \<Longrightarrow> \<Lambda> \<turnstile> \<lparr> f \<rparr>\<^bsub>n\<^esub> \<cdot> v \<leadsto> (f \<cdot> \<lparr> f \<rparr>\<^bsub>n\<^esub> \<bullet> F \<cdot> \<prec>\<^bsub>n\<^esub>) \<cdot> v"
+| ev_ana [simp]: "var\<^sub>t_bind \<Lambda> n = Some F \<Longrightarrow> \<Lambda> \<turnstile> \<lbrakk> f \<rbrakk>\<^bsub>n\<^esub> \<cdot> v \<leadsto> (\<succ>\<^bsub>n\<^esub> \<cdot> \<lbrakk> f \<rbrakk>\<^bsub>n\<^esub> \<bullet> F \<cdot> f) \<cdot> v"
+| ev_var [simp]: "var\<^sub>e_bind \<Lambda> x = Some e \<Longrightarrow> \<Lambda> \<turnstile> Var x \<cdot> v \<leadsto> e \<cdot> v"
 
 (* safety *)
 
-lemma canonical_unit: "\<Gamma> & \<Sigma> \<turnstile> v : \<one> \<Longrightarrow> v = UnitV"
-  by (cases \<Gamma> \<Sigma> v \<one> rule: typecheck\<^sub>v.cases) simp_all
+lemma canonical_unit: "\<Gamma> \<turnstile> v : \<one> \<Longrightarrow> v = UnitV"
+  by (cases \<Gamma> v \<one> rule: typecheck\<^sub>v.cases) simp_all
 
-lemma canonical_prod: "\<Gamma> & \<Sigma> \<turnstile> v : t\<^sub>1 \<otimes> t\<^sub>2 \<Longrightarrow> 
-    \<exists>v\<^sub>1 v\<^sub>2. (\<Gamma> & \<Sigma> \<turnstile> v\<^sub>1 : t\<^sub>1) \<and> (\<Gamma> & \<Sigma> \<turnstile> v\<^sub>2 : t\<^sub>2) \<and> v = PairV v\<^sub>1 v\<^sub>2"
-  by (cases \<Gamma> \<Sigma> v "t\<^sub>1 \<otimes> t\<^sub>2" rule: typecheck\<^sub>v.cases) simp_all
+lemma canonical_prod: "\<Gamma> \<turnstile> v : t\<^sub>1 \<otimes> t\<^sub>2 \<Longrightarrow> \<exists>v\<^sub>1 v\<^sub>2. (\<Gamma> \<turnstile> v\<^sub>1 : t\<^sub>1) \<and> (\<Gamma> \<turnstile> v\<^sub>2 : t\<^sub>2) \<and> v = PairV v\<^sub>1 v\<^sub>2"
+  by (cases \<Gamma> v "t\<^sub>1 \<otimes> t\<^sub>2" rule: typecheck\<^sub>v.cases) simp_all
 
-lemma canonical_sum: "\<Gamma> & \<Sigma> \<turnstile> v : t\<^sub>1 \<oplus> t\<^sub>2 \<Longrightarrow> 
-    \<exists>v'. ((\<Gamma> & \<Sigma> \<turnstile> v' : t\<^sub>1) \<and> v = InlV v') \<or> ((\<Gamma> & \<Sigma> \<turnstile> v' : t\<^sub>2) \<and> v = InrV v')"
-  by (cases \<Gamma> \<Sigma> v "t\<^sub>1 \<oplus> t\<^sub>2" rule: typecheck\<^sub>v.cases) simp_all
+lemma canonical_sum: "\<Gamma> \<turnstile> v : t\<^sub>1 \<oplus> t\<^sub>2 \<Longrightarrow> 
+    \<exists>v'. ((\<Gamma> \<turnstile> v' : t\<^sub>1) \<and> v = InlV v') \<or> ((\<Gamma> \<turnstile> v' : t\<^sub>2) \<and> v = InrV v')"
+  by (cases \<Gamma> v "t\<^sub>1 \<oplus> t\<^sub>2" rule: typecheck\<^sub>v.cases) simp_all
 
-lemma canonical_arrow: "\<Gamma> & \<Sigma> \<turnstile> v : t\<^sub>1 \<hookrightarrow> t\<^sub>2 \<Longrightarrow> \<exists>e. (\<Gamma> & \<Sigma> \<turnstile> e : t\<^sub>1 \<rightarrow> t\<^sub>2) \<and> v = FunV e"
-  by (cases \<Gamma> \<Sigma> v "t\<^sub>1 \<hookrightarrow> t\<^sub>2" rule: typecheck\<^sub>v.cases) simp_all
+lemma canonical_arrow: "\<Gamma> \<turnstile> v : t\<^sub>1 \<hookrightarrow> t\<^sub>2 \<Longrightarrow> \<exists>e. (\<Gamma> \<turnstile> e : t\<^sub>1 \<rightarrow> t\<^sub>2) \<and> v = FunV e"
+  by (cases \<Gamma> v "t\<^sub>1 \<hookrightarrow> t\<^sub>2" rule: typecheck\<^sub>v.cases) simp_all
 
-lemma canonical_mu: "\<Gamma> & \<Sigma> \<turnstile> v : \<mu> F \<Longrightarrow> 
-    \<exists>v' n. (\<Gamma> & \<Sigma> \<turnstile> v' : \<mu> F \<star> F) \<and> v = InjV n v' \<and> \<Sigma> n = Some F"
-  by (cases \<Gamma> \<Sigma> v "\<mu> F" rule: typecheck\<^sub>v.cases) simp_all
+lemma canonical_mu: "\<Gamma> \<turnstile> v : \<mu> F \<Longrightarrow> 
+    \<exists>v' n. (\<Gamma> \<turnstile> v' : \<mu> F \<star> F) \<and> v = InjV n v' \<and> var\<^sub>t_type \<Gamma> n = Some F"
+  by (cases \<Gamma> v "\<mu> F" rule: typecheck\<^sub>v.cases) simp_all
 
-theorem progress [simp]: "\<Gamma> & \<Sigma> \<turnstile> e : t\<^sub>1 \<rightarrow> t\<^sub>2 \<Longrightarrow> \<Gamma> & \<Sigma> \<turnstile> v : t\<^sub>1 \<Longrightarrow> \<Gamma> & \<Sigma> \<tturnstile> \<Lambda> \<Longrightarrow> e \<noteq> \<epsilon> \<Longrightarrow> 
-    \<exists>e' v'. \<Lambda> & \<Sigma> \<turnstile> e \<cdot> v \<leadsto> e' \<cdot> v'"
-    and "\<Gamma> & \<Sigma> \<turnstile> v : t\<^sub>1 \<Longrightarrow> True"
-  proof (induction \<Gamma> \<Sigma> e t\<^sub>1 t\<^sub>2 arbitrary: v rule: typecheck\<^sub>e_typecheck\<^sub>v.inducts)
-  case (tc_con \<Gamma> \<Sigma> v\<^sub>2 t\<^sub>2 t\<^sub>1)
-    have "\<Lambda> & \<Sigma> \<turnstile> \<kappa> v\<^sub>2 \<cdot> v \<leadsto> \<epsilon> \<cdot> v\<^sub>2" by simp
+theorem progress [simp]: "\<Gamma> \<turnstile> e : t\<^sub>1 \<rightarrow> t\<^sub>2 \<Longrightarrow> \<Gamma> \<turnstile> v : t\<^sub>1 \<Longrightarrow> \<Gamma> \<tturnstile> \<Lambda> \<Longrightarrow> e \<noteq> \<epsilon> \<Longrightarrow> 
+    \<exists>e' v'. \<Lambda> \<turnstile> e \<cdot> v \<leadsto> e' \<cdot> v'"
+    and "\<Gamma> \<turnstile> v : t\<^sub>1 \<Longrightarrow> True"
+  proof (induction \<Gamma> e t\<^sub>1 t\<^sub>2 arbitrary: v rule: typecheck\<^sub>e_typecheck\<^sub>v.inducts)
+  case (tc_con \<Gamma> v\<^sub>2 t\<^sub>2 t\<^sub>1)
+    have "\<Lambda> \<turnstile> \<kappa> v\<^sub>2 \<cdot> v \<leadsto> \<epsilon> \<cdot> v\<^sub>2" by simp
     thus ?case by fastforce
-  next case (tc_comp \<Gamma> \<Sigma> f t\<^sub>2 t\<^sub>3 g)
+  next case (tc_comp \<Gamma> f t\<^sub>2 t\<^sub>3 g)
     thus ?case
       proof (cases "g = \<epsilon>")
       case True
-        hence "\<Lambda> & \<Sigma> \<turnstile> (f \<cdot> g) \<cdot> v \<leadsto> f \<cdot> v" by simp
+        hence "\<Lambda> \<turnstile> (f \<cdot> g) \<cdot> v \<leadsto> f \<cdot> v" by simp
         thus ?thesis by fastforce
       next case False
-        with tc_comp obtain g' v' where "\<Lambda> & \<Sigma> \<turnstile> g \<cdot> v \<leadsto> g' \<cdot> v'" by blast
-        with tc_comp have "\<Lambda> & \<Sigma> \<turnstile> (f \<cdot> g) \<cdot> v \<leadsto> (f \<cdot> g') \<cdot> v'" by simp
+        with tc_comp obtain g' v' where "\<Lambda> \<turnstile> g \<cdot> v \<leadsto> g' \<cdot> v'" by blast
+        with tc_comp have "\<Lambda> \<turnstile> (f \<cdot> g) \<cdot> v \<leadsto> (f \<cdot> g') \<cdot> v'" by simp
         thus ?thesis by fastforce
       qed
-  next case (tc_fst \<Gamma> \<Sigma>)
+  next case tc_fst
     then obtain v\<^sub>1 v\<^sub>2 where "v = PairV v\<^sub>1 v\<^sub>2" using canonical_prod by blast
-    hence "\<Lambda> & \<Sigma> \<turnstile> \<pi>\<^sub>1 \<cdot> v \<leadsto> \<epsilon> \<cdot> v\<^sub>1" by simp
+    hence "\<Lambda> \<turnstile> \<pi>\<^sub>1 \<cdot> v \<leadsto> \<epsilon> \<cdot> v\<^sub>1" by simp
     thus ?case by fastforce
-  next case (tc_snd \<Gamma> \<Sigma>)
+  next case tc_snd
     then obtain v\<^sub>1 v\<^sub>2 where "v = PairV v\<^sub>1 v\<^sub>2" using canonical_prod by blast
-    hence "\<Lambda> & \<Sigma> \<turnstile> \<pi>\<^sub>2 \<cdot> v \<leadsto> \<epsilon> \<cdot> v\<^sub>2" by simp
+    hence "\<Lambda> \<turnstile> \<pi>\<^sub>2 \<cdot> v \<leadsto> \<epsilon> \<cdot> v\<^sub>2" by simp
     thus ?case by fastforce
-  next case (tc_tup \<Gamma> \<Sigma>)
-    hence "\<Lambda> & \<Sigma> \<turnstile> \<Theta> \<cdot> v \<leadsto> \<epsilon> \<cdot> PairV v v" by simp
+  next case tc_tup
+    hence "\<Lambda> \<turnstile> \<Theta> \<cdot> v \<leadsto> \<epsilon> \<cdot> PairV v v" by simp
     thus ?case by fastforce
-  next case (tc_pair \<Gamma> \<Sigma> f\<^sub>1 t\<^sub>1 t\<^sub>2 f\<^sub>2)
+  next case (tc_pair \<Gamma> f\<^sub>1 t\<^sub>1 t\<^sub>2 f\<^sub>2)
     then obtain v\<^sub>1 v\<^sub>2 where V: "v = PairV v\<^sub>1 v\<^sub>2" using canonical_prod by blast
     thus ?case
       proof (cases "f\<^sub>1 = \<epsilon>")
@@ -203,334 +244,302 @@ theorem progress [simp]: "\<Gamma> & \<Sigma> \<turnstile> e : t\<^sub>1 \<right
         thus ?thesis
           proof (cases "f\<^sub>2 = \<epsilon>")
           case True
-            have "\<Lambda> & \<Sigma> \<turnstile> \<epsilon> \<parallel> \<epsilon> \<cdot> PairV v\<^sub>1 v\<^sub>2 \<leadsto> \<epsilon> \<cdot> PairV v\<^sub>1 v\<^sub>2" by simp
+            have "\<Lambda> \<turnstile> \<epsilon> \<parallel> \<epsilon> \<cdot> PairV v\<^sub>1 v\<^sub>2 \<leadsto> \<epsilon> \<cdot> PairV v\<^sub>1 v\<^sub>2" by simp
             with T True V show ?thesis by fastforce
           next case False
-            with tc_pair V obtain f\<^sub>2' v\<^sub>2' where "\<Lambda> & \<Sigma> \<turnstile> f\<^sub>2 \<cdot> v\<^sub>2 \<leadsto> f\<^sub>2' \<cdot> v\<^sub>2'" by blast
-            hence "\<Lambda> & \<Sigma> \<turnstile> \<epsilon> \<parallel> f\<^sub>2 \<cdot> PairV v\<^sub>1 v\<^sub>2 \<leadsto> \<epsilon> \<parallel> f\<^sub>2' \<cdot> PairV v\<^sub>1 v\<^sub>2'" by simp
+            with tc_pair V obtain f\<^sub>2' v\<^sub>2' where "\<Lambda> \<turnstile> f\<^sub>2 \<cdot> v\<^sub>2 \<leadsto> f\<^sub>2' \<cdot> v\<^sub>2'" by blast
+            hence "\<Lambda> \<turnstile> \<epsilon> \<parallel> f\<^sub>2 \<cdot> PairV v\<^sub>1 v\<^sub>2 \<leadsto> \<epsilon> \<parallel> f\<^sub>2' \<cdot> PairV v\<^sub>1 v\<^sub>2'" by simp
             with True V show ?thesis by fastforce
           qed
       next case False
-        with tc_pair V obtain f\<^sub>1' v\<^sub>1' where "\<Lambda> & \<Sigma> \<turnstile> f\<^sub>1 \<cdot> v\<^sub>1 \<leadsto> f\<^sub>1' \<cdot> v\<^sub>1'" by blast    
-        hence "\<Lambda> & \<Sigma> \<turnstile> f\<^sub>1 \<parallel> f\<^sub>2 \<cdot> PairV v\<^sub>1 v\<^sub>2 \<leadsto> f\<^sub>1' \<parallel> f\<^sub>2 \<cdot> PairV v\<^sub>1' v\<^sub>2" by simp
+        with tc_pair V obtain f\<^sub>1' v\<^sub>1' where "\<Lambda> \<turnstile> f\<^sub>1 \<cdot> v\<^sub>1 \<leadsto> f\<^sub>1' \<cdot> v\<^sub>1'" by blast    
+        hence "\<Lambda> \<turnstile> f\<^sub>1 \<parallel> f\<^sub>2 \<cdot> PairV v\<^sub>1 v\<^sub>2 \<leadsto> f\<^sub>1' \<parallel> f\<^sub>2 \<cdot> PairV v\<^sub>1' v\<^sub>2" by simp
         with V show ?thesis by fastforce
       qed
-  next case (tc_inl \<Gamma> \<Sigma>)
-    hence "\<Lambda> & \<Sigma> \<turnstile> \<iota>\<^sub>l \<cdot> v \<leadsto> \<epsilon> \<cdot> InlV v" by simp
+  next case tc_inl
+    hence "\<Lambda> \<turnstile> \<iota>\<^sub>l \<cdot> v \<leadsto> \<epsilon> \<cdot> InlV v" by simp
     thus ?case by fastforce
-  next case (tc_inr \<Gamma> \<Sigma>)
-    hence "\<Lambda> & \<Sigma> \<turnstile> \<iota>\<^sub>r \<cdot> v \<leadsto> \<epsilon> \<cdot> InrV v" by simp
+  next case tc_inr
+    hence "\<Lambda> \<turnstile> \<iota>\<^sub>r \<cdot> v \<leadsto> \<epsilon> \<cdot> InrV v" by simp
     thus ?case by fastforce
-  next case (tc_str \<Gamma> \<Sigma>)
+  next case tc_str
     then obtain v' where V: "v = InlV v' \<or> v = InrV v'" using canonical_sum by blast
     thus ?case
       proof (cases "v = InlV v'")
       case True
-        hence "\<Lambda> & \<Sigma> \<turnstile> \<Xi> \<cdot> v \<leadsto> \<epsilon> \<cdot> v'" by simp
+        hence "\<Lambda> \<turnstile> \<Xi> \<cdot> v \<leadsto> \<epsilon> \<cdot> v'" by simp
         thus ?thesis by fastforce
       next case False
-        with V have "\<Lambda> & \<Sigma> \<turnstile> \<Xi> \<cdot> v \<leadsto> \<epsilon> \<cdot> v'" by simp
+        with V have "\<Lambda> \<turnstile> \<Xi> \<cdot> v \<leadsto> \<epsilon> \<cdot> v'" by simp
         thus ?thesis by fastforce
       qed
-  next case (tc_case \<Gamma> \<Sigma> f\<^sub>l t\<^sub>1 t\<^sub>3 f\<^sub>r)
+  next case (tc_case \<Gamma> f\<^sub>l t\<^sub>1 t\<^sub>3 f\<^sub>r)
     then obtain v' where V: "v = InlV v' \<or> v = InrV v'" using canonical_sum by blast
     thus ?case
       proof (cases "v = InlV v'")
       case True
-        hence "\<Lambda> & \<Sigma> \<turnstile> f\<^sub>l \<bar> f\<^sub>r \<cdot> v \<leadsto> (\<iota>\<^sub>l \<cdot> f\<^sub>l) \<cdot> v'" by simp
+        hence "\<Lambda> \<turnstile> f\<^sub>l \<bar> f\<^sub>r \<cdot> v \<leadsto> (\<iota>\<^sub>l \<cdot> f\<^sub>l) \<cdot> v'" by simp
         thus ?thesis by fastforce
       next case False
-        with V have "\<Lambda> & \<Sigma> \<turnstile> f\<^sub>l \<bar> f\<^sub>r \<cdot> v \<leadsto> (\<iota>\<^sub>r \<cdot> f\<^sub>r) \<cdot> v'" by simp
+        with V have "\<Lambda> \<turnstile> f\<^sub>l \<bar> f\<^sub>r \<cdot> v \<leadsto> (\<iota>\<^sub>r \<cdot> f\<^sub>r) \<cdot> v'" by simp
         thus ?thesis by fastforce
       qed
-  next case (tc_dst \<Gamma> \<Sigma>)
+  next case tc_dst
     then obtain v\<^sub>1 v\<^sub>2 where V: "v = PairV (InlV v\<^sub>1) v\<^sub>2 \<or> v = PairV (InrV v\<^sub>1) v\<^sub>2" 
       using canonical_prod canonical_sum by blast
     thus ?case
       proof (cases "v = PairV (InlV v\<^sub>1) v\<^sub>2")
       case True
-        hence "\<Lambda> & \<Sigma> \<turnstile> \<rhd> \<cdot> v \<leadsto> \<epsilon> \<cdot> InlV (PairV v\<^sub>1 v\<^sub>2)" by simp
+        hence "\<Lambda> \<turnstile> \<rhd> \<cdot> v \<leadsto> \<epsilon> \<cdot> InlV (PairV v\<^sub>1 v\<^sub>2)" by simp
         thus ?thesis by fastforce
       next case False
-        with V have "\<Lambda> & \<Sigma> \<turnstile> \<rhd> \<cdot> v \<leadsto> \<epsilon> \<cdot> InrV (PairV v\<^sub>1 v\<^sub>2)" by simp
+        with V have "\<Lambda> \<turnstile> \<rhd> \<cdot> v \<leadsto> \<epsilon> \<cdot> InrV (PairV v\<^sub>1 v\<^sub>2)" by simp
         thus ?thesis by fastforce
       qed
-  next case (tc_app \<Gamma> \<Sigma>)
+  next case tc_app
     then obtain e v' where V: "v = PairV (FunV e) v'" using canonical_prod canonical_arrow by blast
-    moreover hence "\<Lambda> & \<Sigma> \<turnstile> $ \<cdot> v \<leadsto> e \<cdot> v'" by simp
+    moreover hence "\<Lambda> \<turnstile> $ \<cdot> v \<leadsto> e \<cdot> v'" by simp
     ultimately show ?case by fastforce
-  next case (tc_arr \<Gamma> \<Sigma> f t\<^sub>1 t\<^sub>2 g)
+  next case (tc_arr \<Gamma> f t\<^sub>1 t\<^sub>2 g)
     then obtain e where "v = FunV e" using canonical_arrow by blast
-    moreover hence "\<Lambda> & \<Sigma> \<turnstile> g \<leftarrow> f \<cdot> FunV e \<leadsto> \<epsilon> \<cdot> FunV (g \<cdot> e \<cdot> f)" by simp
+    moreover hence "\<Lambda> \<turnstile> g \<leftarrow> f \<cdot> FunV e \<leadsto> \<epsilon> \<cdot> FunV (g \<cdot> e \<cdot> f)" by simp
     ultimately show ?case by fastforce
-  next case (tc_inj \<Sigma> n)
-    hence "\<Lambda> & \<Sigma> \<turnstile> \<succ>\<^bsub>n\<^esub> \<cdot> v \<leadsto> \<epsilon> \<cdot> InjV n v" by simp
+  next case (tc_inj \<Gamma> n)
+    hence "\<Lambda> \<turnstile> \<succ>\<^bsub>n\<^esub> \<cdot> v \<leadsto> \<epsilon> \<cdot> InjV n v" by simp
     thus ?case by fastforce
-  next case (tc_outj \<Sigma> n F \<Gamma>)
-    then obtain v' m where "v = InjV m v' \<and> \<Sigma> m = Some F" using canonical_mu by blast
-    moreover hence "\<Lambda> & \<Sigma> \<turnstile> \<prec>\<^bsub>n\<^esub> \<cdot> v \<leadsto> \<epsilon> \<cdot> v'" by simp
+  next case (tc_outj \<Gamma> n F)
+    then obtain v' m where "v = InjV m v' \<and> var\<^sub>t_type \<Gamma> m = Some F" using canonical_mu by blast
+    moreover hence "\<Lambda> \<turnstile> \<prec>\<^bsub>n\<^esub> \<cdot> v \<leadsto> \<epsilon> \<cdot> v'" by simp
     ultimately show ?case by fastforce
-  next case (tc_cata \<Sigma> n F \<Gamma> f)
-    hence "\<Lambda> & \<Sigma> \<turnstile> \<lparr> f \<rparr>\<^bsub>n\<^esub> \<cdot> v \<leadsto> (f \<cdot> \<lparr> f \<rparr>\<^bsub>n\<^esub> \<bullet> F \<cdot> \<prec>\<^bsub>n\<^esub>) \<cdot> v" by simp
+  next case (tc_cata \<Gamma> n F f t)
+    hence "var\<^sub>t_bind \<Lambda> n = Some F" by (simp add: typecheck_environment_def)
+    hence "\<Lambda> \<turnstile> \<lparr> f \<rparr>\<^bsub>n\<^esub> \<cdot> v \<leadsto> (f \<cdot> \<lparr> f \<rparr>\<^bsub>n\<^esub> \<bullet> F \<cdot> \<prec>\<^bsub>n\<^esub>) \<cdot> v" by simp
     thus ?case by fastforce
-  next case (tc_ana \<Sigma> n F \<Gamma> f)
-    hence "\<Lambda> & \<Sigma> \<turnstile> \<lbrakk> f \<rbrakk>\<^bsub>n\<^esub> \<cdot> v \<leadsto> (\<succ>\<^bsub>n\<^esub> \<cdot> \<lbrakk> f \<rbrakk>\<^bsub>n\<^esub> \<bullet> F \<cdot> f) \<cdot> v" by simp
+  next case (tc_ana \<Gamma> n F f t)
+    hence "var\<^sub>t_bind \<Lambda> n = Some F" by (simp add: typecheck_environment_def)
+    hence "\<Lambda> \<turnstile> \<lbrakk> f \<rbrakk>\<^bsub>n\<^esub> \<cdot> v \<leadsto> (\<succ>\<^bsub>n\<^esub> \<cdot> \<lbrakk> f \<rbrakk>\<^bsub>n\<^esub> \<bullet> F \<cdot> f) \<cdot> v" by simp
     thus ?case by fastforce
-  next case (tc_var \<Gamma> x t\<^sub>1 t\<^sub>2 \<Sigma>)
-    then obtain e where "\<Lambda> x = Some e \<and> \<Gamma> & \<Sigma> \<turnstile> e : t\<^sub>1 \<rightarrow> t\<^sub>2" by (metis typecheck_context_def)
-    hence "\<Lambda> & \<Sigma> \<turnstile> Var x \<cdot> v \<leadsto> e \<cdot> v" by simp
+  next case (tc_var \<Gamma> x t\<^sub>1 t\<^sub>2)
+    then obtain e where "var\<^sub>e_bind \<Lambda> x = Some e \<and> \<Gamma> \<turnstile> e : t\<^sub>1 \<rightarrow> t\<^sub>2" 
+      using typecheck_environment_def by fastforce
+    hence "\<Lambda> \<turnstile> Var x \<cdot> v \<leadsto> e \<cdot> v" by simp
     thus ?case by fastforce
   qed simp_all
 
-lemma [simp]: "\<Gamma> & \<Sigma> \<turnstile> e : t\<^sub>1 \<rightarrow> t\<^sub>2 \<Longrightarrow> \<Gamma> & \<Sigma> \<turnstile> e \<bullet> F : t\<^sub>1 \<star> F \<rightarrow> t\<^sub>2 \<star> F"
+lemma [simp]: "\<Gamma> \<turnstile> e : t\<^sub>1 \<rightarrow> t\<^sub>2 \<Longrightarrow> \<Gamma> \<turnstile> e \<bullet> F : t\<^sub>1 \<star> F \<rightarrow> t\<^sub>2 \<star> F"
   by (induction e F rule: apply_functor_expr.induct) simp_all
 
-theorem preservation [simp]: "\<Lambda> & \<Sigma> \<turnstile> e \<cdot> v \<leadsto> e' \<cdot> v' \<Longrightarrow> \<Gamma> & \<Sigma> \<turnstile> e : t\<^sub>1 \<rightarrow> t\<^sub>2 \<Longrightarrow> 
-    \<Gamma> & \<Sigma> \<turnstile> v : t\<^sub>1 \<Longrightarrow> \<Gamma> & \<Sigma> \<tturnstile> \<Lambda> \<Longrightarrow> \<exists>t\<^sub>3. (\<Gamma> & \<Sigma> \<turnstile> e' : t\<^sub>3 \<rightarrow> t\<^sub>2) \<and> (\<Gamma> & \<Sigma> \<turnstile> v' : t\<^sub>3)"
-  proof (induction \<Lambda> \<Sigma> e v e' v' arbitrary: t\<^sub>1 t\<^sub>2 rule: evaluate.induct)
-  case (ev_pair1 \<Lambda> \<Sigma> f\<^sub>1 v\<^sub>1 f\<^sub>1' v\<^sub>1' f\<^sub>2 v\<^sub>2)
-    then obtain t\<^sub>1\<^sub>1 t\<^sub>1\<^sub>2 t\<^sub>2\<^sub>1 t\<^sub>2\<^sub>2 t\<^sub>1\<^sub>1' where T: "(\<Gamma> & \<Sigma> \<turnstile> v\<^sub>1 : t\<^sub>1\<^sub>1) \<and> (\<Gamma> & \<Sigma> \<turnstile> v\<^sub>2 : t\<^sub>1\<^sub>2) \<and> 
-      (\<Gamma> & \<Sigma> \<turnstile> f\<^sub>1 : t\<^sub>1\<^sub>1 \<rightarrow> t\<^sub>2\<^sub>1) \<and> (\<Gamma> & \<Sigma> \<turnstile> f\<^sub>2 : t\<^sub>1\<^sub>2 \<rightarrow> t\<^sub>2\<^sub>2) \<and> t\<^sub>1 = t\<^sub>1\<^sub>1 \<otimes> t\<^sub>1\<^sub>2 \<and> t\<^sub>2 = t\<^sub>2\<^sub>1 \<otimes> t\<^sub>2\<^sub>2 \<and> 
-        (\<Gamma> & \<Sigma> \<turnstile> f\<^sub>1' : t\<^sub>1\<^sub>1' \<rightarrow> t\<^sub>2\<^sub>1) \<and> \<Gamma> & \<Sigma> \<turnstile> v\<^sub>1' : t\<^sub>1\<^sub>1'" by fastforce
-    hence "(\<Gamma> & \<Sigma> \<turnstile> f\<^sub>1' \<parallel> f\<^sub>2 : t\<^sub>1\<^sub>1' \<otimes> t\<^sub>1\<^sub>2 \<rightarrow> t\<^sub>2) \<and> \<Gamma> & \<Sigma> \<turnstile> PairV v\<^sub>1' v\<^sub>2 : t\<^sub>1\<^sub>1' \<otimes> t\<^sub>1\<^sub>2" by simp
+theorem preservation [simp]: "\<Lambda> \<turnstile> e \<cdot> v \<leadsto> e' \<cdot> v' \<Longrightarrow> \<Gamma> \<turnstile> e : t\<^sub>1 \<rightarrow> t\<^sub>2 \<Longrightarrow> 
+    \<Gamma> \<turnstile> v : t\<^sub>1 \<Longrightarrow> \<Gamma> \<tturnstile> \<Lambda> \<Longrightarrow> \<exists>t\<^sub>3. (\<Gamma> \<turnstile> e' : t\<^sub>3 \<rightarrow> t\<^sub>2) \<and> (\<Gamma> \<turnstile> v' : t\<^sub>3)"
+  proof (induction \<Lambda> e v e' v' arbitrary: t\<^sub>1 t\<^sub>2 rule: evaluate.induct)
+  case (ev_con \<Lambda> v\<^sub>1 v\<^sub>2)
+    hence "(\<Gamma> \<turnstile> \<epsilon> : t\<^sub>2 \<rightarrow> t\<^sub>2) \<and> \<Gamma> \<turnstile> v\<^sub>1 : t\<^sub>2" by fastforce
     thus ?case by fastforce
-  next case (ev_pair2 \<Lambda> \<Sigma> f\<^sub>2 v\<^sub>2 f\<^sub>2' v\<^sub>2' v\<^sub>1)
-    then obtain t\<^sub>1\<^sub>1 t\<^sub>1\<^sub>2 t\<^sub>2\<^sub>2 t\<^sub>1\<^sub>2' where T: "(\<Gamma> & \<Sigma> \<turnstile> v\<^sub>1 : t\<^sub>1\<^sub>1) \<and> (\<Gamma> & \<Sigma> \<turnstile> v\<^sub>2 : t\<^sub>1\<^sub>2) \<and> 
-      (\<Gamma> & \<Sigma> \<turnstile> f\<^sub>2 : t\<^sub>1\<^sub>2 \<rightarrow> t\<^sub>2\<^sub>2) \<and> t\<^sub>1 = t\<^sub>1\<^sub>1 \<otimes> t\<^sub>1\<^sub>2 \<and> t\<^sub>2 = t\<^sub>1\<^sub>1 \<otimes> t\<^sub>2\<^sub>2 \<and> (\<Gamma> & \<Sigma> \<turnstile> f\<^sub>2' : t\<^sub>1\<^sub>2' \<rightarrow> t\<^sub>2\<^sub>2) \<and> 
-        \<Gamma> & \<Sigma> \<turnstile> v\<^sub>2' : t\<^sub>1\<^sub>2'" by fastforce
-    hence "(\<Gamma> & \<Sigma> \<turnstile> \<epsilon> \<parallel> f\<^sub>2' : t\<^sub>1\<^sub>1 \<otimes> t\<^sub>1\<^sub>2' \<rightarrow> t\<^sub>2) \<and> \<Gamma> & \<Sigma> \<turnstile> PairV v\<^sub>1 v\<^sub>2' : t\<^sub>1\<^sub>1 \<otimes> t\<^sub>1\<^sub>2'" by simp
+  next case (ev_comp1 \<Lambda> g v g' v' f)
+    moreover then obtain t\<^sub>3 where "(\<Gamma> \<turnstile> f : t\<^sub>3 \<rightarrow> t\<^sub>2) \<and> \<Gamma> \<turnstile> g : t\<^sub>1 \<rightarrow> t\<^sub>3" by fastforce
+    ultimately obtain t\<^sub>4 where "(\<Gamma> \<turnstile> f \<cdot> g' : t\<^sub>4 \<rightarrow> t\<^sub>2) \<and> \<Gamma> \<turnstile> v' : t\<^sub>4" by fastforce
     thus ?case by fastforce
-  next case (ev_tup \<Lambda> \<Sigma> v)
+  next case (ev_fst \<Lambda> v\<^sub>1 v\<^sub>2)
+    hence "(\<Gamma> \<turnstile> \<epsilon> : t\<^sub>2 \<rightarrow> t\<^sub>2) \<and> \<Gamma> \<turnstile> v\<^sub>1 : t\<^sub>2" by fastforce
+    thus ?case by fastforce
+  next case (ev_snd \<Lambda> v\<^sub>1 v\<^sub>2)
+    hence "(\<Gamma> \<turnstile> \<epsilon> : t\<^sub>2 \<rightarrow> t\<^sub>2) \<and> \<Gamma> \<turnstile> v\<^sub>2 : t\<^sub>2" by fastforce
+    thus ?case by fastforce
+  next case (ev_pair1 \<Lambda> f\<^sub>1 v\<^sub>1 f\<^sub>1' v\<^sub>1' f\<^sub>2 v\<^sub>2)
+    then obtain t\<^sub>1\<^sub>1 t\<^sub>1\<^sub>2 t\<^sub>2\<^sub>1 t\<^sub>2\<^sub>2 t\<^sub>1\<^sub>1' where T: "(\<Gamma> \<turnstile> v\<^sub>1 : t\<^sub>1\<^sub>1) \<and> (\<Gamma> \<turnstile> v\<^sub>2 : t\<^sub>1\<^sub>2) \<and> 
+      (\<Gamma> \<turnstile> f\<^sub>1 : t\<^sub>1\<^sub>1 \<rightarrow> t\<^sub>2\<^sub>1) \<and> (\<Gamma> \<turnstile> f\<^sub>2 : t\<^sub>1\<^sub>2 \<rightarrow> t\<^sub>2\<^sub>2) \<and> t\<^sub>1 = t\<^sub>1\<^sub>1 \<otimes> t\<^sub>1\<^sub>2 \<and> t\<^sub>2 = t\<^sub>2\<^sub>1 \<otimes> t\<^sub>2\<^sub>2 \<and> 
+        (\<Gamma> \<turnstile> f\<^sub>1' : t\<^sub>1\<^sub>1' \<rightarrow> t\<^sub>2\<^sub>1) \<and> \<Gamma> \<turnstile> v\<^sub>1' : t\<^sub>1\<^sub>1'" by fastforce
+    hence "(\<Gamma> \<turnstile> f\<^sub>1' \<parallel> f\<^sub>2 : t\<^sub>1\<^sub>1' \<otimes> t\<^sub>1\<^sub>2 \<rightarrow> t\<^sub>2) \<and> \<Gamma> \<turnstile> PairV v\<^sub>1' v\<^sub>2 : t\<^sub>1\<^sub>1' \<otimes> t\<^sub>1\<^sub>2" by simp
+    thus ?case by fastforce
+  next case (ev_pair2 \<Lambda> f\<^sub>2 v\<^sub>2 f\<^sub>2' v\<^sub>2' v\<^sub>1)
+    then obtain t\<^sub>1\<^sub>1 t\<^sub>1\<^sub>2 t\<^sub>2\<^sub>2 t\<^sub>1\<^sub>2' where T: "(\<Gamma> \<turnstile> v\<^sub>1 : t\<^sub>1\<^sub>1) \<and> (\<Gamma> \<turnstile> v\<^sub>2 : t\<^sub>1\<^sub>2) \<and> 
+      (\<Gamma> \<turnstile> f\<^sub>2 : t\<^sub>1\<^sub>2 \<rightarrow> t\<^sub>2\<^sub>2) \<and> t\<^sub>1 = t\<^sub>1\<^sub>1 \<otimes> t\<^sub>1\<^sub>2 \<and> t\<^sub>2 = t\<^sub>1\<^sub>1 \<otimes> t\<^sub>2\<^sub>2 \<and> (\<Gamma> \<turnstile> f\<^sub>2' : t\<^sub>1\<^sub>2' \<rightarrow> t\<^sub>2\<^sub>2) \<and> 
+        \<Gamma> \<turnstile> v\<^sub>2' : t\<^sub>1\<^sub>2'" by fastforce
+    hence "(\<Gamma> \<turnstile> \<epsilon> \<parallel> f\<^sub>2' : t\<^sub>1\<^sub>1 \<otimes> t\<^sub>1\<^sub>2' \<rightarrow> t\<^sub>2) \<and> \<Gamma> \<turnstile> PairV v\<^sub>1 v\<^sub>2' : t\<^sub>1\<^sub>1 \<otimes> t\<^sub>1\<^sub>2'" by simp
+    thus ?case by fastforce
+  next case (ev_pair3 \<Lambda> v\<^sub>1 v\<^sub>2)
+    hence "(\<Gamma> \<turnstile> \<epsilon> : t\<^sub>1 \<rightarrow> t\<^sub>2) \<and> \<Gamma> \<turnstile> PairV v\<^sub>1 v\<^sub>2 : t\<^sub>1" by fastforce
+    thus ?case by fastforce
+  next case (ev_tup \<Lambda> v)
     hence "t\<^sub>2 = t\<^sub>1 \<otimes> t\<^sub>1" by fastforce
-    moreover from ev_tup have "(\<Gamma> & \<Sigma> \<turnstile> \<epsilon> : t\<^sub>1 \<otimes> t\<^sub>1 \<rightarrow> t\<^sub>1 \<otimes> t\<^sub>1) \<and> \<Gamma> & \<Sigma> \<turnstile> PairV v v : t\<^sub>1 \<otimes> t\<^sub>1" 
+    moreover from ev_tup have "(\<Gamma> \<turnstile> \<epsilon> : t\<^sub>1 \<otimes> t\<^sub>1 \<rightarrow> t\<^sub>1 \<otimes> t\<^sub>1) \<and> \<Gamma> \<turnstile> PairV v v : t\<^sub>1 \<otimes> t\<^sub>1" 
       by simp
     ultimately show ?case by fastforce
-  next case (ev_inl \<Lambda> \<Sigma> v)
+  next case (ev_inl \<Lambda> v)
     moreover then obtain t\<^sub>3 where "t\<^sub>2 = t\<^sub>1 \<oplus> t\<^sub>3" by fastforce
-    ultimately have "(\<Gamma> & \<Sigma> \<turnstile> \<epsilon> : t\<^sub>1 \<oplus> t\<^sub>3 \<rightarrow> t\<^sub>2) \<and> \<Gamma> & \<Sigma> \<turnstile> InlV v : t\<^sub>1 \<oplus> t\<^sub>3" by simp
+    ultimately have "(\<Gamma> \<turnstile> \<epsilon> : t\<^sub>1 \<oplus> t\<^sub>3 \<rightarrow> t\<^sub>2) \<and> \<Gamma> \<turnstile> InlV v : t\<^sub>1 \<oplus> t\<^sub>3" by simp
     thus ?case by fastforce
-  next case (ev_inr \<Lambda> \<Sigma> v)
+  next case (ev_inr \<Lambda> v)
     moreover then obtain t\<^sub>3 where "t\<^sub>2 = t\<^sub>3 \<oplus> t\<^sub>1" by fastforce
-    ultimately have "(\<Gamma> & \<Sigma> \<turnstile> \<epsilon> : t\<^sub>3 \<oplus> t\<^sub>1 \<rightarrow> t\<^sub>2) \<and> \<Gamma> & \<Sigma> \<turnstile> InrV v : t\<^sub>3 \<oplus> t\<^sub>1" by simp
+    ultimately have "(\<Gamma> \<turnstile> \<epsilon> : t\<^sub>3 \<oplus> t\<^sub>1 \<rightarrow> t\<^sub>2) \<and> \<Gamma> \<turnstile> InrV v : t\<^sub>3 \<oplus> t\<^sub>1" by simp
     thus ?case by fastforce
-  next case (ev_csl \<Lambda> \<Sigma> f\<^sub>l f\<^sub>r v)
-    then obtain t\<^sub>1\<^sub>l t\<^sub>1\<^sub>r t\<^sub>2\<^sub>l t\<^sub>2\<^sub>r where V: "(\<Gamma> & \<Sigma> \<turnstile> f\<^sub>l : t\<^sub>1\<^sub>l \<rightarrow> t\<^sub>2\<^sub>l) \<and> (\<Gamma> & \<Sigma> \<turnstile> f\<^sub>r : t\<^sub>1\<^sub>r \<rightarrow> t\<^sub>2\<^sub>r) \<and> 
-      (\<Gamma> & \<Sigma> \<turnstile> v : t\<^sub>1\<^sub>l) \<and> t\<^sub>1 = t\<^sub>1\<^sub>l \<oplus> t\<^sub>1\<^sub>r \<and> t\<^sub>2 = t\<^sub>2\<^sub>l \<oplus> t\<^sub>2\<^sub>r" by fastforce
-    hence "\<Gamma> & \<Sigma> \<turnstile> \<iota>\<^sub>l \<cdot> f\<^sub>l : t\<^sub>1\<^sub>l \<rightarrow> t\<^sub>2\<^sub>l \<oplus> t\<^sub>2\<^sub>r" by (metis tc_inl tc_comp)
+  next case (ev_strl \<Lambda> v)
+    hence "(\<Gamma> \<turnstile> \<epsilon> : t\<^sub>2 \<rightarrow> t\<^sub>2) \<and> \<Gamma> \<turnstile> v : t\<^sub>2" by fastforce
+    thus ?case by fastforce
+  next case (ev_strr \<Lambda> v)
+    hence "(\<Gamma> \<turnstile> \<epsilon> : t\<^sub>2 \<rightarrow> t\<^sub>2) \<and> \<Gamma> \<turnstile> v : t\<^sub>2" by fastforce
+    thus ?case by fastforce
+  next case (ev_csl \<Lambda> f\<^sub>l f\<^sub>r v)
+    then obtain t\<^sub>1\<^sub>l t\<^sub>1\<^sub>r t\<^sub>2\<^sub>l t\<^sub>2\<^sub>r where V: "(\<Gamma> \<turnstile> f\<^sub>l : t\<^sub>1\<^sub>l \<rightarrow> t\<^sub>2\<^sub>l) \<and> (\<Gamma> \<turnstile> f\<^sub>r : t\<^sub>1\<^sub>r \<rightarrow> t\<^sub>2\<^sub>r) \<and> 
+      (\<Gamma> \<turnstile> v : t\<^sub>1\<^sub>l) \<and> t\<^sub>1 = t\<^sub>1\<^sub>l \<oplus> t\<^sub>1\<^sub>r \<and> t\<^sub>2 = t\<^sub>2\<^sub>l \<oplus> t\<^sub>2\<^sub>r" by fastforce
+    hence "\<Gamma> \<turnstile> \<iota>\<^sub>l \<cdot> f\<^sub>l : t\<^sub>1\<^sub>l \<rightarrow> t\<^sub>2\<^sub>l \<oplus> t\<^sub>2\<^sub>r" by (metis tc_inl tc_comp)
     with V show ?case by fastforce
-  next case (ev_csr \<Lambda> \<Sigma> f\<^sub>l f\<^sub>r v)
-    then obtain t\<^sub>1\<^sub>l t\<^sub>1\<^sub>r t\<^sub>2\<^sub>l t\<^sub>2\<^sub>r where V: "(\<Gamma> & \<Sigma> \<turnstile> f\<^sub>l : t\<^sub>1\<^sub>l \<rightarrow> t\<^sub>2\<^sub>l) \<and> (\<Gamma> & \<Sigma> \<turnstile> f\<^sub>r : t\<^sub>1\<^sub>r \<rightarrow> t\<^sub>2\<^sub>r) \<and> 
-      (\<Gamma> & \<Sigma> \<turnstile> v : t\<^sub>1\<^sub>r) \<and> t\<^sub>1 = t\<^sub>1\<^sub>l \<oplus> t\<^sub>1\<^sub>r \<and> t\<^sub>2 = t\<^sub>2\<^sub>l \<oplus> t\<^sub>2\<^sub>r" by fastforce
-    hence "\<Gamma> & \<Sigma> \<turnstile> \<iota>\<^sub>r \<cdot> f\<^sub>r : t\<^sub>1\<^sub>r \<rightarrow> t\<^sub>2\<^sub>l \<oplus> t\<^sub>2\<^sub>r" by (metis tc_inr tc_comp)
+  next case (ev_csr \<Lambda> f\<^sub>l f\<^sub>r v)
+    then obtain t\<^sub>1\<^sub>l t\<^sub>1\<^sub>r t\<^sub>2\<^sub>l t\<^sub>2\<^sub>r where V: "(\<Gamma> \<turnstile> f\<^sub>l : t\<^sub>1\<^sub>l \<rightarrow> t\<^sub>2\<^sub>l) \<and> (\<Gamma> \<turnstile> f\<^sub>r : t\<^sub>1\<^sub>r \<rightarrow> t\<^sub>2\<^sub>r) \<and> 
+      (\<Gamma> \<turnstile> v : t\<^sub>1\<^sub>r) \<and> t\<^sub>1 = t\<^sub>1\<^sub>l \<oplus> t\<^sub>1\<^sub>r \<and> t\<^sub>2 = t\<^sub>2\<^sub>l \<oplus> t\<^sub>2\<^sub>r" by fastforce
+    hence "\<Gamma> \<turnstile> \<iota>\<^sub>r \<cdot> f\<^sub>r : t\<^sub>1\<^sub>r \<rightarrow> t\<^sub>2\<^sub>l \<oplus> t\<^sub>2\<^sub>r" by (metis tc_inr tc_comp)
     with V show ?case by fastforce
-  next case (ev_dstl \<Lambda> \<Sigma> v\<^sub>1 v\<^sub>2)
-    then obtain t\<^sub>3 t\<^sub>4 t\<^sub>5 where "(\<Gamma> & \<Sigma> \<turnstile> v\<^sub>1 : t\<^sub>3) \<and> (\<Gamma> & \<Sigma> \<turnstile> v\<^sub>2 : t\<^sub>5) \<and> t\<^sub>1 = (t\<^sub>3 \<oplus> t\<^sub>4) \<otimes> t\<^sub>5 \<and> 
+  next case (ev_dstl \<Lambda> v\<^sub>1 v\<^sub>2)
+    then obtain t\<^sub>3 t\<^sub>4 t\<^sub>5 where "(\<Gamma> \<turnstile> v\<^sub>1 : t\<^sub>3) \<and> (\<Gamma> \<turnstile> v\<^sub>2 : t\<^sub>5) \<and> t\<^sub>1 = (t\<^sub>3 \<oplus> t\<^sub>4) \<otimes> t\<^sub>5 \<and> 
       t\<^sub>2 = t\<^sub>3 \<otimes> t\<^sub>5 \<oplus> t\<^sub>4 \<otimes> t\<^sub>5" by fastforce
-    hence "(\<Gamma> & \<Sigma> \<turnstile> \<epsilon> : t\<^sub>2 \<rightarrow> t\<^sub>2) \<and> \<Gamma> & \<Sigma> \<turnstile> InlV (PairV v\<^sub>1 v\<^sub>2) : t\<^sub>2" by simp
+    hence "(\<Gamma> \<turnstile> \<epsilon> : t\<^sub>2 \<rightarrow> t\<^sub>2) \<and> \<Gamma> \<turnstile> InlV (PairV v\<^sub>1 v\<^sub>2) : t\<^sub>2" by simp
     thus ?case by fastforce
-  next case (ev_dstr \<Lambda> \<Sigma> v\<^sub>1 v\<^sub>2)
-    then obtain t\<^sub>3 t\<^sub>4 t\<^sub>5 where "(\<Gamma> & \<Sigma> \<turnstile> v\<^sub>1 : t\<^sub>4) \<and> (\<Gamma> & \<Sigma> \<turnstile> v\<^sub>2 : t\<^sub>5) \<and> t\<^sub>1 = (t\<^sub>3 \<oplus> t\<^sub>4) \<otimes> t\<^sub>5 \<and> 
+  next case (ev_dstr \<Lambda> v\<^sub>1 v\<^sub>2)
+    then obtain t\<^sub>3 t\<^sub>4 t\<^sub>5 where "(\<Gamma> \<turnstile> v\<^sub>1 : t\<^sub>4) \<and> (\<Gamma> \<turnstile> v\<^sub>2 : t\<^sub>5) \<and> t\<^sub>1 = (t\<^sub>3 \<oplus> t\<^sub>4) \<otimes> t\<^sub>5 \<and> 
       t\<^sub>2 = t\<^sub>3 \<otimes> t\<^sub>5 \<oplus> t\<^sub>4 \<otimes> t\<^sub>5" by fastforce
-    hence "(\<Gamma> & \<Sigma> \<turnstile> \<epsilon> : t\<^sub>2 \<rightarrow> t\<^sub>2) \<and> \<Gamma> & \<Sigma> \<turnstile> InrV (PairV v\<^sub>1 v\<^sub>2) : t\<^sub>2" by simp
+    hence "(\<Gamma> \<turnstile> \<epsilon> : t\<^sub>2 \<rightarrow> t\<^sub>2) \<and> \<Gamma> \<turnstile> InrV (PairV v\<^sub>1 v\<^sub>2) : t\<^sub>2" by simp
     thus ?case by fastforce
-  next case (ev_arr \<Lambda> \<Sigma> g f e)
-    then obtain t\<^sub>1\<^sub>1 t\<^sub>1\<^sub>2 t\<^sub>2\<^sub>1 t\<^sub>2\<^sub>2 where "(\<Gamma> & \<Sigma> \<turnstile> f : t\<^sub>2\<^sub>1 \<rightarrow> t\<^sub>1\<^sub>1) \<and> (\<Gamma> & \<Sigma> \<turnstile> g : t\<^sub>1\<^sub>2 \<rightarrow> t\<^sub>2\<^sub>2) \<and> 
-      (\<Gamma> & \<Sigma> \<turnstile> e : t\<^sub>1\<^sub>1 \<rightarrow> t\<^sub>1\<^sub>2) \<and> t\<^sub>1 = t\<^sub>1\<^sub>1 \<hookrightarrow> t\<^sub>1\<^sub>2 \<and> t\<^sub>2 = t\<^sub>2\<^sub>1 \<hookrightarrow> t\<^sub>2\<^sub>2" by fastforce
-    hence "(\<Gamma> & \<Sigma> \<turnstile> \<epsilon> : t\<^sub>2\<^sub>1 \<hookrightarrow> t\<^sub>2\<^sub>2 \<rightarrow> t\<^sub>2) \<and> \<Gamma> & \<Sigma> \<turnstile> FunV (g \<cdot> e \<cdot> f) : t\<^sub>2\<^sub>1 \<hookrightarrow> t\<^sub>2\<^sub>2" by fastforce
+  next case (ev_arr \<Lambda> g f e)
+    then obtain t\<^sub>1\<^sub>1 t\<^sub>1\<^sub>2 t\<^sub>2\<^sub>1 t\<^sub>2\<^sub>2 where "(\<Gamma> \<turnstile> f : t\<^sub>2\<^sub>1 \<rightarrow> t\<^sub>1\<^sub>1) \<and> (\<Gamma> \<turnstile> g : t\<^sub>1\<^sub>2 \<rightarrow> t\<^sub>2\<^sub>2) \<and> 
+      (\<Gamma> \<turnstile> e : t\<^sub>1\<^sub>1 \<rightarrow> t\<^sub>1\<^sub>2) \<and> t\<^sub>1 = t\<^sub>1\<^sub>1 \<hookrightarrow> t\<^sub>1\<^sub>2 \<and> t\<^sub>2 = t\<^sub>2\<^sub>1 \<hookrightarrow> t\<^sub>2\<^sub>2" by fastforce
+    hence "(\<Gamma> \<turnstile> \<epsilon> : t\<^sub>2\<^sub>1 \<hookrightarrow> t\<^sub>2\<^sub>2 \<rightarrow> t\<^sub>2) \<and> \<Gamma> \<turnstile> FunV (g \<cdot> e \<cdot> f) : t\<^sub>2\<^sub>1 \<hookrightarrow> t\<^sub>2\<^sub>2" by fastforce
     thus ?case by fastforce
-  next case (ev_inj \<Lambda> \<Sigma> F v)
-    hence "(\<Gamma> & \<Sigma> \<turnstile> \<epsilon> : t\<^sub>2 \<rightarrow> t\<^sub>2) \<and> \<Gamma> & \<Sigma> \<turnstile> InjV F v : t\<^sub>2" by fastforce
+  next case (ev_inj \<Lambda> F v)
+    hence "(\<Gamma> \<turnstile> \<epsilon> : t\<^sub>2 \<rightarrow> t\<^sub>2) \<and> \<Gamma> \<turnstile> InjV F v : t\<^sub>2" by fastforce
     thus ?case by fastforce
-  next case (ev_cata \<Sigma> n F \<Lambda> f v)
-    hence V: "(\<Gamma> & \<Sigma> \<turnstile> f : t\<^sub>2 \<star> F \<rightarrow> t\<^sub>2) \<and> \<Gamma> & \<Sigma> \<turnstile> v : \<mu> F" by fastforce
-    moreover from ev_cata have "\<Gamma> & \<Sigma> \<turnstile> \<lparr> f \<rparr>\<^bsub>n\<^esub> \<bullet> F : \<mu> F \<star> F \<rightarrow> t\<^sub>2 \<star> F" by fastforce
-    moreover from ev_cata have "\<Gamma> & \<Sigma> \<turnstile> \<prec>\<^bsub>n\<^esub> : \<mu> F \<rightarrow> \<mu> F \<star> F" by simp
-    ultimately have "\<Gamma> & \<Sigma> \<turnstile> f \<cdot> \<lparr> f \<rparr>\<^bsub>n\<^esub> \<bullet> F \<cdot> \<prec>\<^bsub>n\<^esub> : \<mu> F \<rightarrow> t\<^sub>2" by (metis tc_comp)
-    with V have "(\<Gamma> & \<Sigma> \<turnstile> f \<cdot> \<lparr> f \<rparr>\<^bsub>n\<^esub> \<bullet> F \<cdot> \<prec>\<^bsub>n\<^esub> : \<mu> F \<rightarrow> t\<^sub>2) \<and> \<Gamma> & \<Sigma> \<turnstile> v : \<mu> F" by simp
+  next case (ev_outj \<Lambda> m F v)
+    hence "(\<Gamma> \<turnstile> \<epsilon> : t\<^sub>2 \<rightarrow> t\<^sub>2) \<and> \<Gamma> \<turnstile> v : t\<^sub>2" by fastforce
     thus ?case by fastforce
-  next case (ev_ana \<Sigma> n F \<Lambda> f v)
-    moreover hence V: "(\<Gamma> & \<Sigma> \<turnstile> f : t\<^sub>1 \<rightarrow> t\<^sub>1 \<star> F) \<and> (\<Gamma> & \<Sigma> \<turnstile> v : t\<^sub>1) \<and> t\<^sub>2 = \<mu> F" by fastforce
-    ultimately have "\<Gamma> & \<Sigma> \<turnstile> \<succ>\<^bsub>n\<^esub> : t\<^sub>2 \<star> F \<rightarrow> t\<^sub>2" by simp
-    moreover from ev_ana have "\<Gamma> & \<Sigma> \<turnstile> \<lbrakk> f \<rbrakk>\<^bsub>n\<^esub> \<bullet> F : t\<^sub>1 \<star> F \<rightarrow> t\<^sub>2 \<star> F" by simp
-    moreover from V have "\<Gamma> & \<Sigma> \<turnstile> f : t\<^sub>1 \<rightarrow> t\<^sub>1 \<star> F" by simp
-    ultimately have "\<Gamma> & \<Sigma> \<turnstile> \<succ>\<^bsub>n\<^esub> \<cdot> \<lbrakk> f \<rbrakk>\<^bsub>n\<^esub> \<bullet> F \<cdot> f : t\<^sub>1 \<rightarrow> t\<^sub>2" by simp
+  next case (ev_cata \<Lambda> n F f v)
+    hence V: "(\<Gamma> \<turnstile> f : t\<^sub>2 \<star> F \<rightarrow> t\<^sub>2) \<and> \<Gamma> \<turnstile> v : \<mu> F" using typecheck_environment_def by fastforce
+    moreover from ev_cata have "\<Gamma> \<turnstile> \<lparr> f \<rparr>\<^bsub>n\<^esub> \<bullet> F : \<mu> F \<star> F \<rightarrow> t\<^sub>2 \<star> F" 
+      using typecheck_environment_def by fastforce
+    moreover from ev_cata have "\<Gamma> \<turnstile> \<prec>\<^bsub>n\<^esub> : \<mu> F \<rightarrow> \<mu> F \<star> F" using typecheck_environment_def by simp
+    ultimately have "\<Gamma> \<turnstile> f \<cdot> \<lparr> f \<rparr>\<^bsub>n\<^esub> \<bullet> F \<cdot> \<prec>\<^bsub>n\<^esub> : \<mu> F \<rightarrow> t\<^sub>2" by (metis tc_comp)
+    with V have "(\<Gamma> \<turnstile> f \<cdot> \<lparr> f \<rparr>\<^bsub>n\<^esub> \<bullet> F \<cdot> \<prec>\<^bsub>n\<^esub> : \<mu> F \<rightarrow> t\<^sub>2) \<and> \<Gamma> \<turnstile> v : \<mu> F" by simp
+    thus ?case by fastforce
+  next case (ev_ana \<Lambda> n F f v)
+    moreover hence V: "(\<Gamma> \<turnstile> f : t\<^sub>1 \<rightarrow> t\<^sub>1 \<star> F) \<and> (\<Gamma> \<turnstile> v : t\<^sub>1) \<and> t\<^sub>2 = \<mu> F"
+      using typecheck_environment_def by fastforce
+    ultimately have "\<Gamma> \<turnstile> \<succ>\<^bsub>n\<^esub> : t\<^sub>2 \<star> F \<rightarrow> t\<^sub>2" using typecheck_environment_def by simp
+    moreover from ev_ana have "\<Gamma> \<turnstile> \<lbrakk> f \<rbrakk>\<^bsub>n\<^esub> \<bullet> F : t\<^sub>1 \<star> F \<rightarrow> t\<^sub>2 \<star> F" by simp
+    moreover from V have "\<Gamma> \<turnstile> f : t\<^sub>1 \<rightarrow> t\<^sub>1 \<star> F" by simp
+    ultimately have "\<Gamma> \<turnstile> \<succ>\<^bsub>n\<^esub> \<cdot> \<lbrakk> f \<rbrakk>\<^bsub>n\<^esub> \<bullet> F \<cdot> f : t\<^sub>1 \<rightarrow> t\<^sub>2" by simp
     with V show ?case by fastforce
-  next case (ev_var \<Lambda> x e \<Sigma> v)
-    hence "\<Gamma> x = Some (t\<^sub>1, t\<^sub>2)" by fastforce
-    with ev_var obtain e' where "\<Lambda> x = Some e' \<and> \<Gamma> & \<Sigma> \<turnstile> e' : t\<^sub>1 \<rightarrow> t\<^sub>2" 
-      by (metis typecheck_context_def)
+  next case (ev_var \<Lambda> x e v)
+    hence "var\<^sub>e_type \<Gamma> x = Some (t\<^sub>1, t\<^sub>2)" by fastforce
+    with ev_var obtain e' where "var\<^sub>e_bind \<Lambda> x = Some e' \<and> \<Gamma> \<turnstile> e' : t\<^sub>1 \<rightarrow> t\<^sub>2" 
+      using typecheck_environment_def by fastforce 
     with ev_var show ?case by fastforce
-  qed force+
+  qed fastforce+
 
 (* big-step evaluation *) 
 
-inductive total_eval :: "(name \<rightharpoonup> expr) \<Rightarrow> (name \<rightharpoonup> funct) \<Rightarrow> expr \<Rightarrow> val \<Rightarrow> val \<Rightarrow> bool" 
-    (infix "& _ \<turnstile> _ \<cdot> _ \<Down>" 60) where
-  tev_base [simp]: "\<Lambda> & \<Sigma> \<turnstile> \<epsilon> \<cdot> v \<Down> v"
-| tev_step [simp]: "\<Lambda> & \<Sigma> \<turnstile> e \<cdot> v \<leadsto> e' \<cdot> v' \<Longrightarrow> \<Lambda> & \<Sigma> \<turnstile> e' \<cdot> v' \<Down> v'' \<Longrightarrow> \<Lambda> & \<Sigma> \<turnstile> e \<cdot> v \<Down> v''"
+inductive total_eval :: "dynamic_environment \<Rightarrow> expr \<Rightarrow> val \<Rightarrow> val \<Rightarrow> bool" 
+    (infix "\<turnstile> _ \<cdot> _ \<Down>" 60) where
+  tev_base [simp]: "\<Lambda> \<turnstile> \<epsilon> \<cdot> v \<Down> v"
+| tev_step [simp]: "\<Lambda> \<turnstile> e \<cdot> v \<leadsto> e' \<cdot> v' \<Longrightarrow> \<Lambda> \<turnstile> e' \<cdot> v' \<Down> v'' \<Longrightarrow> \<Lambda> \<turnstile> e \<cdot> v \<Down> v''"
 
-lemma [elim]: "\<Lambda> & \<Sigma> \<turnstile> f \<cdot> v \<Down> v' \<Longrightarrow> \<Lambda> & \<Sigma> \<turnstile> g \<cdot> v' \<Down> v'' \<Longrightarrow> \<Lambda> & \<Sigma> \<turnstile> (g \<cdot> f) \<cdot> v \<Down> v''"
-  proof (induction \<Lambda> \<Sigma> f v v' rule: total_eval.induct)
-  case (tev_base \<Lambda> \<Sigma> v)
-    moreover have "\<Lambda> & \<Sigma> \<turnstile> (g \<cdot> \<epsilon>) \<cdot> v \<leadsto> g \<cdot> v" by simp
+lemma [elim]: "\<Lambda> \<turnstile> f \<cdot> v \<Down> v' \<Longrightarrow> \<Lambda> \<turnstile> g \<cdot> v' \<Down> v'' \<Longrightarrow> \<Lambda> \<turnstile> (g \<cdot> f) \<cdot> v \<Down> v''"
+  proof (induction \<Lambda> f v v' rule: total_eval.induct)
+  case (tev_base \<Lambda> v)
+    moreover have "\<Lambda> \<turnstile> (g \<cdot> \<epsilon>) \<cdot> v \<leadsto> g \<cdot> v" by simp
     ultimately show ?case by (metis tev_step)
-  next case (tev_step \<Lambda> \<Sigma> f v f' v' v''')
-    hence "\<Lambda> & \<Sigma> \<turnstile> (g \<cdot> f) \<cdot> v \<leadsto> (g \<cdot> f') \<cdot> v'" by simp
-    moreover from tev_step have "\<Lambda> & \<Sigma> \<turnstile> (g \<cdot> f') \<cdot> v' \<Down> v''" by simp
+  next case (tev_step \<Lambda> f v f' v' v''')
+    hence "\<Lambda> \<turnstile> (g \<cdot> f) \<cdot> v \<leadsto> (g \<cdot> f') \<cdot> v'" by simp
+    moreover from tev_step have "\<Lambda> \<turnstile> (g \<cdot> f') \<cdot> v' \<Down> v''" by simp
     ultimately show ?case by (metis total_eval.tev_step)
   qed
 
-lemma [simp]: "\<Lambda> & \<Sigma> \<turnstile> e \<cdot> v \<leadsto> \<epsilon> \<cdot> v' \<Longrightarrow> \<Lambda> & \<Sigma> \<turnstile> e \<cdot> v \<Down> v'"
+lemma [simp]: "\<Lambda> \<turnstile> e \<cdot> v \<leadsto> \<epsilon> \<cdot> v' \<Longrightarrow> \<Lambda> \<turnstile> e \<cdot> v \<Down> v'"
   by rule (simp, simp)
 
-lemma eps_big_eval [elim]: "\<Lambda> & \<Sigma> \<turnstile> \<epsilon> \<cdot> v \<Down> v' \<Longrightarrow> v = v'"
-  proof (induction \<Lambda> \<Sigma> \<epsilon> v v' rule: total_eval.induct)
-  case (tev_step \<Lambda> \<Sigma> v e' v' v'')
+lemma eps_big_eval [elim]: "\<Lambda> \<turnstile> \<epsilon> \<cdot> v \<Down> v' \<Longrightarrow> v = v'"
+  proof (induction \<Lambda> \<epsilon> v v' rule: total_eval.induct)
+  case (tev_step \<Lambda> v e' v' v'')
     thus ?case by (induction \<epsilon> v e' v' rule: evaluate.induct)
   qed simp_all
 
-lemma [simp]: "\<Lambda> & \<Sigma> \<turnstile> f\<^sub>2 \<cdot> v\<^sub>2 \<Down> v\<^sub>4 \<Longrightarrow> \<Lambda> & \<Sigma> \<turnstile> \<epsilon> \<parallel> f\<^sub>2 \<cdot> PairV v\<^sub>1 v\<^sub>2 \<Down> PairV v\<^sub>1 v\<^sub>4"
-  proof (induction \<Lambda> \<Sigma> f\<^sub>2 v\<^sub>2 v\<^sub>4 rule: total_eval.induct)
-  case (tev_step \<Lambda> \<Sigma> f\<^sub>2 v\<^sub>2 f\<^sub>2' v\<^sub>2' v\<^sub>4)
-    hence "\<Lambda> & \<Sigma> \<turnstile> \<epsilon> \<parallel> f\<^sub>2 \<cdot> PairV v\<^sub>1 v\<^sub>2 \<leadsto> \<epsilon> \<parallel> f\<^sub>2' \<cdot> PairV v\<^sub>1 v\<^sub>2'" by simp
-    moreover from tev_step have "\<Lambda> & \<Sigma> \<turnstile> \<epsilon> \<parallel> f\<^sub>2' \<cdot> PairV v\<^sub>1 v\<^sub>2' \<Down> PairV v\<^sub>1 v\<^sub>4" by simp
+lemma [simp]: "\<Lambda> \<turnstile> f\<^sub>2 \<cdot> v\<^sub>2 \<Down> v\<^sub>4 \<Longrightarrow> \<Lambda> \<turnstile> \<epsilon> \<parallel> f\<^sub>2 \<cdot> PairV v\<^sub>1 v\<^sub>2 \<Down> PairV v\<^sub>1 v\<^sub>4"
+  proof (induction \<Lambda> f\<^sub>2 v\<^sub>2 v\<^sub>4 rule: total_eval.induct)
+  case (tev_step \<Lambda> f\<^sub>2 v\<^sub>2 f\<^sub>2' v\<^sub>2' v\<^sub>4)
+    hence "\<Lambda> \<turnstile> \<epsilon> \<parallel> f\<^sub>2 \<cdot> PairV v\<^sub>1 v\<^sub>2 \<leadsto> \<epsilon> \<parallel> f\<^sub>2' \<cdot> PairV v\<^sub>1 v\<^sub>2'" by simp
+    moreover from tev_step have "\<Lambda> \<turnstile> \<epsilon> \<parallel> f\<^sub>2' \<cdot> PairV v\<^sub>1 v\<^sub>2' \<Down> PairV v\<^sub>1 v\<^sub>4" by simp
     ultimately show ?case by simp
   qed simp_all
 
-lemma [simp]: "\<Lambda> & \<Sigma> \<turnstile> f\<^sub>1 \<cdot> v\<^sub>1 \<Down> v\<^sub>3 \<Longrightarrow> \<Lambda> & \<Sigma> \<turnstile> f\<^sub>2 \<cdot> v\<^sub>2 \<Down> v\<^sub>4 \<Longrightarrow> 
-    \<Lambda> & \<Sigma> \<turnstile> f\<^sub>1 \<parallel> f\<^sub>2 \<cdot> PairV v\<^sub>1 v\<^sub>2 \<Down> PairV v\<^sub>3 v\<^sub>4"
-  proof (induction \<Lambda> \<Sigma> f\<^sub>1 v\<^sub>1 v\<^sub>3 rule: total_eval.induct)
-  case (tev_step \<Lambda> \<Sigma> f\<^sub>1 v\<^sub>1 f\<^sub>1' v\<^sub>1' v\<^sub>3)
-    hence "\<Lambda> & \<Sigma> \<turnstile> f\<^sub>1 \<parallel> f\<^sub>2 \<cdot> PairV v\<^sub>1 v\<^sub>2 \<leadsto> f\<^sub>1' \<parallel> f\<^sub>2 \<cdot> PairV v\<^sub>1' v\<^sub>2" by simp
-    moreover from tev_step have "\<Lambda> & \<Sigma> \<turnstile> f\<^sub>1' \<parallel> f\<^sub>2 \<cdot> PairV v\<^sub>1' v\<^sub>2 \<Down> PairV v\<^sub>3 v\<^sub>4" by simp
+lemma [simp]: "\<Lambda> \<turnstile> f\<^sub>1 \<cdot> v\<^sub>1 \<Down> v\<^sub>3 \<Longrightarrow> \<Lambda> \<turnstile> f\<^sub>2 \<cdot> v\<^sub>2 \<Down> v\<^sub>4 \<Longrightarrow> 
+    \<Lambda> \<turnstile> f\<^sub>1 \<parallel> f\<^sub>2 \<cdot> PairV v\<^sub>1 v\<^sub>2 \<Down> PairV v\<^sub>3 v\<^sub>4"
+  proof (induction \<Lambda> f\<^sub>1 v\<^sub>1 v\<^sub>3 rule: total_eval.induct)
+  case (tev_step \<Lambda> f\<^sub>1 v\<^sub>1 f\<^sub>1' v\<^sub>1' v\<^sub>3)
+    hence "\<Lambda> \<turnstile> f\<^sub>1 \<parallel> f\<^sub>2 \<cdot> PairV v\<^sub>1 v\<^sub>2 \<leadsto> f\<^sub>1' \<parallel> f\<^sub>2 \<cdot> PairV v\<^sub>1' v\<^sub>2" by simp
+    moreover from tev_step have "\<Lambda> \<turnstile> f\<^sub>1' \<parallel> f\<^sub>2 \<cdot> PairV v\<^sub>1' v\<^sub>2 \<Down> PairV v\<^sub>3 v\<^sub>4" by simp
     ultimately show ?case by simp
   qed simp_all
 
-lemma pair_big_eval [elim]: "\<Lambda> & \<Sigma> \<turnstile> f\<^sub>1 \<parallel> f\<^sub>2 \<cdot> PairV v\<^sub>1 v\<^sub>2 \<Down> PairV v\<^sub>3 v\<^sub>4 \<Longrightarrow> 
-    (\<Lambda> & \<Sigma> \<turnstile> f\<^sub>1 \<cdot> v\<^sub>1 \<Down> v\<^sub>3) \<and> \<Lambda> & \<Sigma> \<turnstile> f\<^sub>2 \<cdot> v\<^sub>2 \<Down> v\<^sub>4"
-  proof (induction \<Lambda> \<Sigma> "f\<^sub>1 \<parallel> f\<^sub>2" "PairV v\<^sub>1 v\<^sub>2" "PairV v\<^sub>3 v\<^sub>4" 
+lemma pair_big_eval [elim]: "\<Lambda> \<turnstile> f\<^sub>1 \<parallel> f\<^sub>2 \<cdot> PairV v\<^sub>1 v\<^sub>2 \<Down> PairV v\<^sub>3 v\<^sub>4 \<Longrightarrow> 
+    (\<Lambda> \<turnstile> f\<^sub>1 \<cdot> v\<^sub>1 \<Down> v\<^sub>3) \<and> \<Lambda> \<turnstile> f\<^sub>2 \<cdot> v\<^sub>2 \<Down> v\<^sub>4"
+  proof (induction \<Lambda> "f\<^sub>1 \<parallel> f\<^sub>2" "PairV v\<^sub>1 v\<^sub>2" "PairV v\<^sub>3 v\<^sub>4" 
          arbitrary: f\<^sub>1 f\<^sub>2 v\<^sub>1 v\<^sub>2 rule: total_eval.induct)
-  case (tev_step \<Lambda> \<Sigma> e' v')
+  case (tev_step \<Lambda> e' v')
     thus ?case
-      proof (induction \<Lambda> \<Sigma> "f\<^sub>1 \<parallel> f\<^sub>2" "PairV v\<^sub>1 v\<^sub>2" e' v' arbitrary: f\<^sub>1 f\<^sub>2 v\<^sub>1 v\<^sub>2 rule: evaluate.induct)
-      case (ev_pair3 \<Lambda> \<Sigma> v\<^sub>1 v\<^sub>2)
+      proof (induction \<Lambda> "f\<^sub>1 \<parallel> f\<^sub>2" "PairV v\<^sub>1 v\<^sub>2" e' v' arbitrary: f\<^sub>1 f\<^sub>2 v\<^sub>1 v\<^sub>2 rule: evaluate.induct)
+      case (ev_pair3 \<Lambda> v\<^sub>1 v\<^sub>2)
         hence "PairV v\<^sub>1 v\<^sub>2 = PairV v\<^sub>3 v\<^sub>4" by (metis eps_big_eval)
         thus ?case by simp
       qed simp_all
   qed
 
-lemma [simp]: "\<Lambda> & \<Sigma> \<turnstile> f\<^sub>l \<cdot> v \<Down> v' \<Longrightarrow> \<Lambda> & \<Sigma> \<turnstile> f\<^sub>l \<bar> f\<^sub>r \<cdot> InlV v \<Down> InlV v'"
+lemma [simp]: "\<Lambda> \<turnstile> f\<^sub>l \<cdot> v \<Down> v' \<Longrightarrow> \<Lambda> \<turnstile> f\<^sub>l \<bar> f\<^sub>r \<cdot> InlV v \<Down> InlV v'"
   proof
-    show "\<Lambda> & \<Sigma> \<turnstile> f\<^sub>l \<bar> f\<^sub>r \<cdot> InlV v \<leadsto> (\<iota>\<^sub>l \<cdot> f\<^sub>l) \<cdot> v" by simp
-    show "\<Lambda> & \<Sigma> \<turnstile> f\<^sub>l \<cdot> v \<Down> v' \<Longrightarrow> \<Lambda> & \<Sigma> \<turnstile> (\<iota>\<^sub>l \<cdot> f\<^sub>l) \<cdot> v \<Down> InlV v'" by auto
+    show "\<Lambda> \<turnstile> f\<^sub>l \<bar> f\<^sub>r \<cdot> InlV v \<leadsto> (\<iota>\<^sub>l \<cdot> f\<^sub>l) \<cdot> v" by simp
+    show "\<Lambda> \<turnstile> f\<^sub>l \<cdot> v \<Down> v' \<Longrightarrow> \<Lambda> \<turnstile> (\<iota>\<^sub>l \<cdot> f\<^sub>l) \<cdot> v \<Down> InlV v'" by auto
   qed
 
-lemma [simp]: "\<Lambda> & \<Sigma> \<turnstile> f\<^sub>r \<cdot> v \<Down> v' \<Longrightarrow> \<Lambda> & \<Sigma> \<turnstile> f\<^sub>l \<bar> f\<^sub>r \<cdot> InrV v \<Down> InrV v'"
+lemma [simp]: "\<Lambda> \<turnstile> f\<^sub>r \<cdot> v \<Down> v' \<Longrightarrow> \<Lambda> \<turnstile> f\<^sub>l \<bar> f\<^sub>r \<cdot> InrV v \<Down> InrV v'"
   proof
-    show "\<Lambda> & \<Sigma> \<turnstile> f\<^sub>l \<bar> f\<^sub>r \<cdot> InrV v \<leadsto> (\<iota>\<^sub>r \<cdot> f\<^sub>r) \<cdot> v" by simp
-    show "\<Lambda> & \<Sigma> \<turnstile> f\<^sub>r \<cdot> v \<Down> v' \<Longrightarrow> \<Lambda> & \<Sigma> \<turnstile> (\<iota>\<^sub>r \<cdot> f\<^sub>r) \<cdot> v \<Down> InrV v'" by auto
+    show "\<Lambda> \<turnstile> f\<^sub>l \<bar> f\<^sub>r \<cdot> InrV v \<leadsto> (\<iota>\<^sub>r \<cdot> f\<^sub>r) \<cdot> v" by simp
+    show "\<Lambda> \<turnstile> f\<^sub>r \<cdot> v \<Down> v' \<Longrightarrow> \<Lambda> \<turnstile> (\<iota>\<^sub>r \<cdot> f\<^sub>r) \<cdot> v \<Down> InrV v'" by auto
   qed
 
 (* since we are a turing-complete language, total progress is not provable *)
 
-theorem total_preservation [simp]: "\<Lambda> & \<Sigma> \<turnstile> e \<cdot> v \<Down> v' \<Longrightarrow> \<Gamma> & \<Sigma> \<turnstile> e : t\<^sub>1 \<rightarrow> t\<^sub>2 \<Longrightarrow> 
-    \<Gamma> & \<Sigma> \<turnstile> v : t\<^sub>1 \<Longrightarrow> \<Gamma> & \<Sigma> \<tturnstile> \<Lambda> \<Longrightarrow> \<Gamma> & \<Sigma> \<turnstile> v' : t\<^sub>2"
-  proof (induction \<Lambda> \<Sigma> e v v' arbitrary: t\<^sub>1 rule: total_eval.induct)
-  case (tev_step \<Lambda> \<Sigma> e v e' v' v'')
-    moreover then obtain t\<^sub>3 where "(\<Gamma> & \<Sigma> \<turnstile> e' : t\<^sub>3 \<rightarrow> t\<^sub>2) \<and> (\<Gamma> & \<Sigma> \<turnstile> v' : t\<^sub>3)" 
+theorem total_preservation [simp]: "\<Lambda> \<turnstile> e \<cdot> v \<Down> v' \<Longrightarrow> \<Gamma> \<turnstile> e : t\<^sub>1 \<rightarrow> t\<^sub>2 \<Longrightarrow> 
+    \<Gamma> \<turnstile> v : t\<^sub>1 \<Longrightarrow> \<Gamma> \<tturnstile> \<Lambda> \<Longrightarrow> \<Gamma> \<turnstile> v' : t\<^sub>2"
+  proof (induction \<Lambda> e v v' arbitrary: t\<^sub>1 rule: total_eval.induct)
+  case (tev_step \<Lambda> e v e' v' v'')
+    moreover then obtain t\<^sub>3 where "(\<Gamma> \<turnstile> e' : t\<^sub>3 \<rightarrow> t\<^sub>2) \<and> (\<Gamma> \<turnstile> v' : t\<^sub>3)" 
       by (metis preservation)
     ultimately show ?case by fastforce
   qed auto
 
-(* misc lemmas *)
+(* environment lemmas *)
 
-lemma [simp]: "\<Gamma> & \<Sigma> \<turnstile> e : t\<^sub>1 \<rightarrow> t\<^sub>2 \<Longrightarrow> x \<notin> dom \<Gamma> \<Longrightarrow> \<Gamma>(x \<mapsto> tt) & \<Sigma> \<turnstile> e : t\<^sub>1 \<rightarrow> t\<^sub>2"
-  and [simp]: "\<Gamma> & \<Sigma> \<turnstile> v : t \<Longrightarrow> x \<notin> dom \<Gamma> \<Longrightarrow> \<Gamma>(x \<mapsto> tt) & \<Sigma> \<turnstile> v : t"
-  proof (induction \<Gamma> \<Sigma> e t\<^sub>1 t\<^sub>2 and \<Gamma> \<Sigma> v t rule: typecheck\<^sub>e_typecheck\<^sub>v.inducts) 
-  case (tc_var \<Gamma> y t\<^sub>1 t\<^sub>2)
-    moreover hence "x \<noteq> y" by auto
-    ultimately show ?case by simp
-  qed simp_all
+lemma [simp]: "\<Gamma> \<turnstile> e : t\<^sub>1 \<rightarrow> t\<^sub>2 \<Longrightarrow> x \<notin> domain\<^sub>s \<Gamma> \<Longrightarrow> extend\<^sub>e\<^sub>s x tt \<Gamma> \<turnstile> e : t\<^sub>1 \<rightarrow> t\<^sub>2"
+  and [simp]: "\<Gamma> \<turnstile> v : t \<Longrightarrow> x \<notin> domain\<^sub>s \<Gamma> \<Longrightarrow> extend\<^sub>e\<^sub>s x tt \<Gamma> \<turnstile> v : t"
+  by (induction \<Gamma> e t\<^sub>1 t\<^sub>2 and \<Gamma> v t rule: typecheck\<^sub>e_typecheck\<^sub>v.inducts) simp_all
 
-lemma [simp]: "\<Gamma> & \<Sigma> \<turnstile> e : t\<^sub>1 \<rightarrow> t\<^sub>2 \<Longrightarrow> \<Gamma>' ++ \<Gamma> & \<Sigma> \<turnstile> e : t\<^sub>1 \<rightarrow> t\<^sub>2"
-  and [simp]: "\<Gamma> & \<Sigma> \<turnstile> v : t \<Longrightarrow> \<Gamma>' ++ \<Gamma> & \<Sigma> \<turnstile> v : t"
-  by (induction \<Gamma> \<Sigma> e t\<^sub>1 t\<^sub>2 and \<Gamma> \<Sigma> v t rule: typecheck\<^sub>e_typecheck\<^sub>v.inducts) simp_all
+lemma [simp]: "\<Gamma> \<turnstile> e : t\<^sub>1 \<rightarrow> t\<^sub>2 \<Longrightarrow> x \<notin> domain\<^sub>s \<Gamma> \<Longrightarrow> extend\<^sub>v\<^sub>s x t \<Gamma> \<turnstile> e : t\<^sub>1 \<rightarrow> t\<^sub>2"
+  and [simp]: "\<Gamma> \<turnstile> v : t \<Longrightarrow> x \<notin> domain\<^sub>s \<Gamma> \<Longrightarrow> extend\<^sub>v\<^sub>s x t \<Gamma> \<turnstile> v : t"
+  by (induction \<Gamma> e t\<^sub>1 t\<^sub>2 and \<Gamma> v t rule: typecheck\<^sub>e_typecheck\<^sub>v.inducts) simp_all
 
-lemma [simp]: "\<Gamma> & \<Sigma> \<turnstile> e : t\<^sub>1 \<rightarrow> t\<^sub>2 \<Longrightarrow> dom \<Gamma> \<inter> dom \<Gamma>' = {} \<Longrightarrow> \<Gamma> ++ \<Gamma>' & \<Sigma> \<turnstile> e : t\<^sub>1 \<rightarrow> t\<^sub>2"
-  and [simp]: "\<Gamma> & \<Sigma> \<turnstile> v : t \<Longrightarrow> dom \<Gamma> \<inter> dom \<Gamma>' = {} \<Longrightarrow> \<Gamma> ++ \<Gamma>' & \<Sigma> \<turnstile> v : t"
-  proof (induction \<Gamma> \<Sigma> e t\<^sub>1 t\<^sub>2 and \<Gamma> \<Sigma> v t rule: typecheck\<^sub>e_typecheck\<^sub>v.inducts) 
-  case (tc_var \<Gamma> x t\<^sub>1 t\<^sub>2 \<Sigma>)
-    moreover hence "\<Gamma>' x = None" by auto
-    ultimately show ?case by (simp add: map_add_def)
-  qed simp_all
+lemma [simp]: "\<Gamma> \<turnstile> e : t\<^sub>1 \<rightarrow> t\<^sub>2 \<Longrightarrow> combine\<^sub>s \<Gamma>' \<Gamma> \<turnstile> e : t\<^sub>1 \<rightarrow> t\<^sub>2"
+  and [simp]: "\<Gamma> \<turnstile> v : t \<Longrightarrow> combine\<^sub>s \<Gamma>' \<Gamma> \<turnstile> v : t"
+  by (induction \<Gamma> e t\<^sub>1 t\<^sub>2 and \<Gamma> v t rule: typecheck\<^sub>e_typecheck\<^sub>v.inducts) simp_all
 
-lemma [simp]: "\<Gamma> & \<Sigma> \<turnstile> e : t\<^sub>1 \<rightarrow> t\<^sub>2 \<Longrightarrow> x \<notin> dom \<Sigma> \<Longrightarrow> \<Gamma> & \<Sigma>(x \<mapsto> F) \<turnstile> e : t\<^sub>1 \<rightarrow> t\<^sub>2"
-  and [simp]: "\<Gamma> & \<Sigma> \<turnstile> v : t \<Longrightarrow> x \<notin> dom \<Sigma> \<Longrightarrow> \<Gamma> & \<Sigma>(x \<mapsto> F) \<turnstile> v : t"
-  proof (induction \<Gamma> \<Sigma> e t\<^sub>1 t\<^sub>2 and \<Gamma> \<Sigma> v t rule: typecheck\<^sub>e_typecheck\<^sub>v.inducts)
-  case (tc_inj \<Sigma> n F' \<Gamma>)
-    hence "(\<Sigma>(x \<mapsto> F)) n = Some F'" by auto
-    thus ?case by simp
-  next case (tc_outj \<Sigma> n F' \<Gamma>)
-    hence "(\<Sigma>(x \<mapsto> F)) n = Some F'" by auto
-    thus ?case by simp
-  next case (tc_cata \<Sigma> n F' \<Gamma>)
-    moreover hence "(\<Sigma>(x \<mapsto> F)) n = Some F'" by auto
-    ultimately show ?case by simp
-  next case (tc_ana \<Sigma> n F' \<Gamma>)
-    moreover hence "(\<Sigma>(x \<mapsto> F)) n = Some F'" by auto
-    ultimately show ?case by simp
-  next case (tcv_inj \<Sigma> n F' \<Gamma>)
-    moreover hence "(\<Sigma>(x \<mapsto> F)) n = Some F'" by auto
-    ultimately show ?case by simp
-  qed simp_all
+lemma [simp]: "\<Gamma> \<turnstile> e : t\<^sub>1 \<rightarrow> t\<^sub>2 \<Longrightarrow> domain\<^sub>s \<Gamma> \<inter> domain\<^sub>s \<Gamma>' = {} \<Longrightarrow> combine\<^sub>s \<Gamma> \<Gamma>' \<turnstile> e : t\<^sub>1 \<rightarrow> t\<^sub>2"
+  and [simp]: "\<Gamma> \<turnstile> v : t \<Longrightarrow> domain\<^sub>s \<Gamma> \<inter> domain\<^sub>s \<Gamma>' = {} \<Longrightarrow> combine\<^sub>s \<Gamma> \<Gamma>' \<turnstile> v : t"
+  by (induction \<Gamma> e t\<^sub>1 t\<^sub>2 and \<Gamma> v t rule: typecheck\<^sub>e_typecheck\<^sub>v.inducts) simp_all
 
-lemma [simp]: "\<Gamma> & \<Sigma> \<tturnstile> \<Lambda> \<Longrightarrow> x \<notin> dom \<Sigma> \<Longrightarrow> \<Gamma> & \<Sigma>(x \<mapsto> F) \<tturnstile> \<Lambda>"
-  proof (unfold typecheck_context_def, rule, rule, rule, rule)
-    fix y t\<^sub>1 t\<^sub>2
-    assume "\<forall>x t\<^sub>1 t\<^sub>2. \<Gamma> x = Some (t\<^sub>1, t\<^sub>2) \<longrightarrow> (\<exists>e. \<Lambda> x = Some e \<and> \<Gamma> & \<Sigma> \<turnstile> e : t\<^sub>1 \<rightarrow> t\<^sub>2)"
-       and "\<Gamma> y = Some (t\<^sub>1, t\<^sub>2)"
-    then obtain e where "\<Lambda> y = Some e \<and> \<Gamma> & \<Sigma> \<turnstile> e : t\<^sub>1 \<rightarrow> t\<^sub>2" by blast
-    moreover assume "x \<notin> dom \<Sigma>"
-    ultimately show "\<exists>e. \<Lambda> y = Some e \<and> \<Gamma> & \<Sigma>(x \<mapsto> F) \<turnstile> e : t\<^sub>1 \<rightarrow> t\<^sub>2" by simp
-  qed
+lemma [simp]: "\<Gamma> \<turnstile> e : t\<^sub>1 \<rightarrow> t\<^sub>2 \<Longrightarrow> \<Gamma> \<tturnstile> \<Lambda> \<Longrightarrow> x \<notin> domain\<^sub>s \<Gamma> \<Longrightarrow> 
+    extend\<^sub>e\<^sub>s x (t\<^sub>1, t\<^sub>2) \<Gamma> \<tturnstile> extend\<^sub>e\<^sub>d x e \<Lambda>"
+  by simp
 
-lemma [simp]: "\<Gamma> & \<Sigma> \<turnstile> e : t\<^sub>1 \<rightarrow> t\<^sub>2 \<Longrightarrow> \<Gamma> & \<Sigma> \<tturnstile> \<Lambda> \<Longrightarrow> x \<notin> dom \<Lambda> \<Longrightarrow> 
-    \<Gamma>(x \<mapsto> (t\<^sub>1, t\<^sub>2)) & \<Sigma> \<tturnstile> \<Lambda>(x \<mapsto> e)"
-  proof (unfold typecheck_context_def, rule, rule, rule, rule)
-    fix y t\<^sub>1' t\<^sub>2'
-    assume A: "\<Gamma> & \<Sigma> \<turnstile> e : t\<^sub>1 \<rightarrow> t\<^sub>2"
-       and B: "\<forall>x t\<^sub>1 t\<^sub>2. \<Gamma> x = Some (t\<^sub>1, t\<^sub>2) \<longrightarrow> (\<exists>e. \<Lambda> x = Some e \<and> \<Gamma> & \<Sigma> \<turnstile> e : t\<^sub>1 \<rightarrow> t\<^sub>2)"
-       and C: "x \<notin> dom \<Lambda>"
-       and D: "(\<Gamma>(x \<mapsto> (t\<^sub>1, t\<^sub>2))) y = Some (t\<^sub>1', t\<^sub>2')"
-    moreover hence E: "x \<notin> dom \<Gamma>" by auto
-    ultimately show "\<exists>e'. (\<Lambda>(x \<mapsto> e)) y = Some e' \<and> \<Gamma>(x \<mapsto> (t\<^sub>1, t\<^sub>2)) & \<Sigma> \<turnstile> e' : t\<^sub>1' \<rightarrow> t\<^sub>2'"
-      proof (cases "x = y")
-      case False
-        with B D obtain e' where "\<Lambda> y = Some e' \<and> \<Gamma> & \<Sigma> \<turnstile> e' : t\<^sub>1' \<rightarrow> t\<^sub>2'" by fastforce
-        with E False show ?thesis by simp
-      qed simp_all
-  qed
+lemma [simp]: "\<Gamma> \<turnstile> v : t \<Longrightarrow> \<Gamma> \<tturnstile> \<Lambda> \<Longrightarrow> x \<notin> domain\<^sub>s \<Gamma> \<Longrightarrow> extend\<^sub>v\<^sub>s x t \<Gamma> \<tturnstile> extend\<^sub>v\<^sub>d x v \<Lambda>"
+  by simp
 
-lemma [simp]: "\<Gamma> & \<Sigma> \<tturnstile> \<Lambda> \<Longrightarrow> \<Gamma>' & \<Sigma> \<tturnstile> \<Lambda>' \<Longrightarrow> dom \<Gamma> \<inter> dom \<Gamma>' = {} \<Longrightarrow> dom \<Lambda> \<inter> dom \<Lambda>' = {} \<Longrightarrow> 
-    \<Gamma> ++ \<Gamma>' & \<Sigma> \<tturnstile> \<Lambda> ++ \<Lambda>'"
-  proof (unfold typecheck_context_def, rule, rule, rule, rule)
-    fix x t\<^sub>1 t\<^sub>2
-    assume A: "\<forall>x t\<^sub>1 t\<^sub>2. \<Gamma> x = Some (t\<^sub>1, t\<^sub>2) \<longrightarrow> (\<exists>e. \<Lambda> x = Some e \<and> \<Gamma> & \<Sigma> \<turnstile> e : t\<^sub>1 \<rightarrow> t\<^sub>2)"
-    assume B: "\<forall>x t\<^sub>1 t\<^sub>2. \<Gamma>' x = Some (t\<^sub>1, t\<^sub>2) \<longrightarrow> (\<exists>e. \<Lambda>' x = Some e \<and> \<Gamma>' & \<Sigma> \<turnstile> e : t\<^sub>1 \<rightarrow> t\<^sub>2)"
-    assume C: "dom \<Gamma> \<inter> dom \<Gamma>' = {}"
-    assume D: "dom \<Lambda> \<inter> dom \<Lambda>' = {}"
-    assume E: "(\<Gamma> ++ \<Gamma>') x = Some (t\<^sub>1, t\<^sub>2)"
-    show "\<exists>e. (\<Lambda> ++ \<Lambda>') x = Some e \<and> \<Gamma> ++ \<Gamma>' & \<Sigma> \<turnstile> e : t\<^sub>1 \<rightarrow> t\<^sub>2" 
-      proof (cases "x \<in> dom \<Gamma>'")
-      case True
-        with B E obtain e where "\<Lambda>' x = Some e \<and> \<Gamma>' & \<Sigma> \<turnstile> e : t\<^sub>1 \<rightarrow> t\<^sub>2" by fastforce
-        thus ?thesis by simp
-      next case False
-        with A E obtain e where F: "\<Lambda> x = Some e \<and> \<Gamma> & \<Sigma> \<turnstile> e : t\<^sub>1 \<rightarrow> t\<^sub>2" by fastforce
-        with D have "\<Lambda>' x = None" by auto
-        with F have "(\<Lambda> ++ \<Lambda>') x = Some e" by (simp add: map_add_def)
-        with C F show ?thesis by simp
-      qed
-  qed
+lemma [simp]: "\<Gamma> \<tturnstile> \<Lambda> \<Longrightarrow> \<Gamma>' \<tturnstile> \<Lambda>' \<Longrightarrow> domain\<^sub>s \<Gamma> \<inter> domain\<^sub>s \<Gamma>' = {} \<Longrightarrow> 
+    combine\<^sub>s \<Gamma> \<Gamma>' \<tturnstile> combine\<^sub>d \<Lambda> \<Lambda>'"
+  by simp
 
 end
